ExpressionSemantics/Expression_Syntax.thy
@@ -141,9 +141,9 @@ where
   \<open>e1 lt e2 = (BinOp e1 (LOp Lt) e2)\<close>
 
 fun 
-  lteq_exp :: \<open>exp \<Rightarrow> exp \<Rightarrow> exp\<close>
+  le_exp :: \<open>exp \<Rightarrow> exp \<Rightarrow> exp\<close>
 where
-  \<open>e1 lteq e2 = (BinOp e1 (LOp Le) e2)\<close>
+  \<open>e1 le e2 = (BinOp e1 (LOp Le) e2)\<close>
 
 fun 
   slt_exp :: \<open>exp \<Rightarrow> exp \<Rightarrow> exp\<close>
@@ -151,9 +151,9 @@ where
   \<open>e1 slt e2 = (BinOp e1 (LOp Slt) e2)\<close>
 
 fun 
-  slteq_exp :: \<open>exp \<Rightarrow> exp \<Rightarrow> exp\<close>
+  sle_exp :: \<open>exp \<Rightarrow> exp \<Rightarrow> exp\<close>
 where
-  \<open>e1 slteq e2 = (BinOp e1 (LOp Sle) e2)\<close>
+  \<open>e1 sle e2 = (BinOp e1 (LOp Sle) e2)\<close>
 
 fun 
   uminus_exp :: \<open>exp \<Rightarrow> exp\<close>
@@ -169,8 +169,6 @@ fun
   plus_exp :: \<open>exp \<Rightarrow> exp \<Rightarrow> exp\<close>
 where
   \<open>plus_exp e1 e2 = (BinOp e1 (AOp Plus) e2)\<close>
-
-declare plus_exp.simps[simp del]
 
 fun 
   times_exp :: \<open>exp \<Rightarrow> exp \<Rightarrow> exp\<close>
@@ -848,83 +846,758 @@ fun
 where
   \<open>(\<Delta> \<turnstile> e \<leadsto>* v) = (v = eval_exp \<Delta> e)\<close>
 
-(*
+
 inductive
   eval_exp' :: \<open>variables \<Rightarrow> exp \<Rightarrow> exp \<Rightarrow> bool\<close> (\<open>_ \<turnstile> _ \<Rrightarrow> _\<close> [400, 400, 400] 401)
 where
-  VarIn: \<open>\<lbrakk>((name' :\<^sub>t t), val) \<in>\<^sub>\<Delta> \<Delta>\<rbrakk> \<Longrightarrow> (\<Delta> \<turnstile> (name' :\<^sub>t t) \<Rrightarrow> Val val)\<close> |
-  VarNotIn: \<open>\<lbrakk>((name' :\<^sub>t t)) \<notin> dom \<Delta>\<rbrakk> \<Longrightarrow> (\<Delta> \<turnstile> (name' :\<^sub>t t) \<Rrightarrow> unknown[str]: t)\<close> |
-  LoadStepAddr: \<open>\<lbrakk>\<Delta> \<turnstile> e\<^sub>2 \<Rrightarrow> e\<^sub>2'; e\<^sub>2 \<noteq> e\<^sub>2'\<rbrakk> \<Longrightarrow> (\<Delta> \<turnstile> e\<^sub>1[e\<^sub>2, ed]:usz \<Rrightarrow> (e\<^sub>1[e\<^sub>2', ed]:usz))\<close> |
-  LoadStepMem: \<open>\<lbrakk>\<Delta> \<turnstile> e\<^sub>1 \<Rrightarrow> e\<^sub>1'; e\<^sub>1 \<noteq> e\<^sub>1'\<rbrakk> \<Longrightarrow> (\<Delta> \<turnstile> e\<^sub>1[Val v\<^sub>2, ed]:usz \<Rrightarrow> (e\<^sub>1'[Val v\<^sub>2, ed]:usz))\<close>
+  \<comment> \<open>Var rules\<close>
+  VarIn: \<open>\<lbrakk>((name' :\<^sub>t t), val) \<in>\<^sub>\<Delta> \<Delta>\<rbrakk> \<Longrightarrow> \<Delta> \<turnstile> (name' :\<^sub>t t) \<Rrightarrow> Val val\<close> |
+  VarNotIn: \<open>\<lbrakk>((name' :\<^sub>t t)) \<notin> dom \<Delta>\<rbrakk> \<Longrightarrow> \<Delta> \<turnstile> (name' :\<^sub>t t) \<Rrightarrow> unknown[str]: t\<close> |
 
-lemma step_exp_var_inE:
-  assumes \<open>\<Delta> \<turnstile> (name' :\<^sub>t t) \<Rrightarrow> e'\<close>
-      and \<open>((name' :\<^sub>t t), val) \<in>\<^sub>\<Delta> \<Delta>\<close>
-    shows \<open>e' = Val val\<close>
-using assms(1) proof (cases rule: eval_exp'.cases)
-  case (VarIn name' t val)
-  then show ?thesis sorry
+  \<comment> \<open>Load\<close>
+  LoadStepAddr: \<open>\<lbrakk>\<Delta> \<turnstile> e\<^sub>2 \<Rrightarrow> e\<^sub>2'; e\<^sub>2 \<noteq> e\<^sub>2'\<rbrakk> \<Longrightarrow> \<Delta> \<turnstile> e\<^sub>1[e\<^sub>2, ed]:usz \<Rrightarrow> (e\<^sub>1[e\<^sub>2', ed]:usz)\<close> |
+  LoadStepMem: \<open>\<lbrakk>\<Delta> \<turnstile> e\<^sub>1 \<Rrightarrow> e\<^sub>1'; e\<^sub>1 \<noteq> e\<^sub>1'\<rbrakk> \<Longrightarrow> \<Delta> \<turnstile> e\<^sub>1[Val v\<^sub>2, ed]:usz \<Rrightarrow> (e\<^sub>1'[Val v\<^sub>2, ed]:usz)\<close> |
+  LoadByte: \<open>\<Delta> \<turnstile> v[(num \<Colon> sz\<^sub>a\<^sub>d\<^sub>d\<^sub>r) \<leftarrow> v', sz][(num \<Colon> sz\<^sub>a\<^sub>d\<^sub>d\<^sub>r), ed]:usz \<Rrightarrow> Val v'\<close> | 
+  LoadByteFromNext: \<open>\<lbrakk>((num\<^sub>1 \<Colon> sz\<^sub>1)::word) \<noteq> (num\<^sub>2 \<Colon> sz\<^sub>2)\<rbrakk> \<Longrightarrow> \<Delta> \<turnstile> ((v[(num\<^sub>1 \<Colon> sz\<^sub>1) \<leftarrow> v', sz][(num\<^sub>2 \<Colon> sz\<^sub>2), ed]:usz)::exp) \<Rrightarrow> ((Val v)[(num\<^sub>2 \<Colon> sz\<^sub>2), ed]:usz)\<close> |
+  LoadUnMem: \<open>\<Delta> \<turnstile> (unknown[str]: t)[Val v, ed]:usz \<Rrightarrow> unknown[str]: imm\<langle>sz\<rangle>\<close> |
+  LoadUnAddr: \<open>\<Delta> \<turnstile> v[w \<leftarrow> v', sz][unknown[str]: t, ed]:usz' \<Rrightarrow> unknown[str]: imm\<langle>sz'\<rangle>\<close> |
+  LoadWordBe: \<open>\<lbrakk>sz > sz\<^sub>m\<^sub>e\<^sub>m; type v = mem\<langle>sz\<^sub>a\<^sub>d\<^sub>d\<^sub>r, sz\<^sub>m\<^sub>e\<^sub>m\<rangle>\<rbrakk> \<Longrightarrow> 
+      \<Delta> \<turnstile> ((Val v)[(num \<Colon> sz\<^sub>a\<^sub>d\<^sub>d\<^sub>r), be]:usz) \<Rrightarrow> (((Val v)[(num \<Colon> sz\<^sub>a\<^sub>d\<^sub>d\<^sub>r), be]:usz\<^sub>m\<^sub>e\<^sub>m) @ (((Val v)[succ (num \<Colon> sz\<^sub>a\<^sub>d\<^sub>d\<^sub>r), be]:u(sz - sz\<^sub>m\<^sub>e\<^sub>m))))\<close> |
+  LoadWordEl: \<open>\<lbrakk>sz > sz\<^sub>m\<^sub>e\<^sub>m; type v = mem\<langle>sz\<^sub>a\<^sub>d\<^sub>d\<^sub>r, sz\<^sub>m\<^sub>e\<^sub>m\<rangle>\<rbrakk> \<Longrightarrow> 
+      \<Delta> \<turnstile> ((Val v)[(num \<Colon> sz\<^sub>a\<^sub>d\<^sub>d\<^sub>r), el]:usz) \<Rrightarrow> ((((Val v)[succ (num \<Colon> sz\<^sub>a\<^sub>d\<^sub>d\<^sub>r), el]:u(sz - sz\<^sub>m\<^sub>e\<^sub>m))) @ ((Val v)[(num \<Colon> sz\<^sub>a\<^sub>d\<^sub>d\<^sub>r), el]:usz\<^sub>m\<^sub>e\<^sub>m))\<close> |
+
+  \<comment> \<open>Store\<close>
+  StoreStepVal: \<open>\<Delta> \<turnstile> e\<^sub>3 \<Rrightarrow> e\<^sub>3' \<Longrightarrow> \<Delta> \<turnstile> (e\<^sub>1 with [e\<^sub>2, en]:usz \<leftarrow> e\<^sub>3) \<Rrightarrow> (e\<^sub>1 with [e\<^sub>2, en]:usz \<leftarrow> e\<^sub>3')\<close> |
+  StoreStepAddr: \<open>\<Delta> \<turnstile> e\<^sub>2 \<Rrightarrow> e\<^sub>2' \<Longrightarrow> \<Delta> \<turnstile> (e\<^sub>1 with [e\<^sub>2, en]:usz \<leftarrow> (Val v\<^sub>3)) \<Rrightarrow> (e\<^sub>1 with [e\<^sub>2', en]:usz \<leftarrow> (Val v\<^sub>3))\<close> |
+  StoreStepMem: \<open>\<Delta> \<turnstile> e\<^sub>1 \<Rrightarrow> e\<^sub>1' \<Longrightarrow> \<Delta> \<turnstile> (e\<^sub>1 with [(Val v\<^sub>2), en]:usz \<leftarrow> (Val v\<^sub>3)) \<Rrightarrow> (e\<^sub>1' with [(Val v\<^sub>2), en]:usz \<leftarrow> (Val v\<^sub>3))\<close> |
+  StoreWordBe: \<open>\<lbrakk>sz\<^sub>m\<^sub>e\<^sub>m < sz; type v = mem\<langle>sz\<^sub>a\<^sub>d\<^sub>d\<^sub>r, sz\<^sub>m\<^sub>e\<^sub>m\<rangle>; e\<^sub>1 = ((Val v) with [(num \<Colon> sz\<^sub>a\<^sub>d\<^sub>d\<^sub>r), be]:usz\<^sub>m\<^sub>e\<^sub>m \<leftarrow> (Cast High sz\<^sub>m\<^sub>e\<^sub>m (Val val)))\<rbrakk> \<Longrightarrow>
+    \<Delta> \<turnstile> ((Val v) with [(num \<Colon> sz\<^sub>a\<^sub>d\<^sub>d\<^sub>r), be]:usz \<leftarrow> (Val val)) \<Rrightarrow> (e\<^sub>1 with [(succ (num \<Colon> sz\<^sub>a\<^sub>d\<^sub>d\<^sub>r)), be]:u(sz - sz\<^sub>m\<^sub>e\<^sub>m) \<leftarrow> (Cast Low (sz - sz\<^sub>m\<^sub>e\<^sub>m) (Val val)))\<close> |
+  StoreWordEl: \<open>\<lbrakk>sz\<^sub>m\<^sub>e\<^sub>m < sz; type v = mem\<langle>sz\<^sub>a\<^sub>d\<^sub>d\<^sub>r, sz\<^sub>m\<^sub>e\<^sub>m\<rangle>; e\<^sub>1 = ((Val v) with [(num \<Colon> sz\<^sub>a\<^sub>d\<^sub>d\<^sub>r), el]:usz\<^sub>m\<^sub>e\<^sub>m \<leftarrow> (Cast Low sz\<^sub>m\<^sub>e\<^sub>m (Val val)))\<rbrakk> \<Longrightarrow>
+    \<Delta> \<turnstile> ((Val v) with [(num \<Colon> sz\<^sub>a\<^sub>d\<^sub>d\<^sub>r), el]:usz \<leftarrow> (Val val)) \<Rrightarrow> (e\<^sub>1 with [(succ (num \<Colon> sz\<^sub>a\<^sub>d\<^sub>d\<^sub>r)), el]:u(sz - sz\<^sub>m\<^sub>e\<^sub>m) \<leftarrow> (Cast High (sz - sz\<^sub>m\<^sub>e\<^sub>m) (Val val)))\<close> |
+  StoreVal: \<open>type v = mem\<langle>sz\<^sub>a\<^sub>d\<^sub>d\<^sub>r, sz\<^sub>m\<^sub>e\<^sub>m\<rangle> \<Longrightarrow> \<Delta> \<turnstile> ((Val v) with [(num \<Colon> sz\<^sub>a\<^sub>d\<^sub>d\<^sub>r), ed]:usz\<^sub>m\<^sub>e\<^sub>m \<leftarrow> (Val v')) \<Rrightarrow> (v[(num \<Colon> sz\<^sub>a\<^sub>d\<^sub>d\<^sub>r) \<leftarrow> v', sz\<^sub>m\<^sub>e\<^sub>m])\<close> |
+  StoreUnAddr: \<open>type v = t \<Longrightarrow> \<Delta> \<turnstile> ((Val v) with [unknown[str]: imm\<langle>sz\<^sub>a\<^sub>d\<^sub>d\<^sub>r\<rangle>, ed]:usz' \<leftarrow> (Val v')) \<Rrightarrow> (unknown[str]: t)\<close> |
+
+
+  \<comment> \<open>Let rules\<close>
+  LetStep: \<open>\<Delta> \<turnstile> e\<^sub>1 \<Rrightarrow> e\<^sub>1' \<Longrightarrow> \<Delta> \<turnstile> (Let var e\<^sub>1 e\<^sub>2) \<Rrightarrow> (Let var e\<^sub>1' e\<^sub>2)\<close> |
+  (* one missing rule *)
+
+  \<comment> \<open>If rules\<close>
+  IfStepCond: \<open>\<Delta> \<turnstile> e\<^sub>1 \<Rrightarrow> e\<^sub>1'\<Longrightarrow> \<Delta> \<turnstile> (ite e\<^sub>1 (Val v\<^sub>2) (Val v\<^sub>3)) \<Rrightarrow> ite e\<^sub>1' (Val v\<^sub>2) (Val v\<^sub>3)\<close> |
+  IfStepThen: \<open>\<Delta> \<turnstile> e\<^sub>2 \<Rrightarrow> e\<^sub>2'\<Longrightarrow> \<Delta> \<turnstile> (ite e\<^sub>1 e\<^sub>2 (Val v\<^sub>3)) \<Rrightarrow> ite e\<^sub>1 e\<^sub>2' (Val v\<^sub>3)\<close> |
+  IfStepElse: \<open>\<Delta> \<turnstile> e\<^sub>3 \<Rrightarrow> e\<^sub>3'\<Longrightarrow> \<Delta> \<turnstile> (ite e\<^sub>1 e\<^sub>2 e\<^sub>3) \<Rrightarrow> ite e\<^sub>1 e\<^sub>2 e\<^sub>3'\<close> |
+  IfTrue: \<open>\<Delta> \<turnstile> (ite true (Val v\<^sub>2) (Val v\<^sub>3)) \<Rrightarrow> (Val v\<^sub>2)\<close> |
+  IfFalse: \<open>\<Delta> \<turnstile> (ite false (Val v\<^sub>2) (Val v\<^sub>3)) \<Rrightarrow> (Val v\<^sub>3)\<close> |
+  IfUnknown: \<open>\<lbrakk>type v\<^sub>2 = t'\<rbrakk> \<Longrightarrow> \<Delta> \<turnstile> (ite unknown[str]: t (Val v\<^sub>2) (Val v\<^sub>3)) \<Rrightarrow> unknown[str]: t'\<close> |
+
+  \<comment> \<open>Binary operation rules\<close>
+  BopRhs: \<open>\<Delta> \<turnstile> e\<^sub>2 \<Rrightarrow> e\<^sub>2' \<Longrightarrow> \<Delta> \<turnstile> BinOp (Val v) bop e\<^sub>2 \<Rrightarrow> BinOp (Val v) bop e\<^sub>2'\<close> |
+  BopLhs: \<open>\<Delta> \<turnstile> e\<^sub>1 \<Rrightarrow> e\<^sub>1' \<Longrightarrow> \<Delta> \<turnstile> BinOp e\<^sub>1 bop e\<^sub>2 \<Rrightarrow> BinOp e\<^sub>1' bop e\<^sub>2\<close> |
+
+  AopUnkRhs: \<open>\<Delta> \<turnstile> BinOp (unknown[str]: t) (AOp aop) e \<Rrightarrow> unknown[str]: t\<close> |
+  AopUnkLhs: \<open>\<Delta> \<turnstile> BinOp e (AOp aop) (unknown[str]: t) \<Rrightarrow> unknown[str]: t\<close> |
+
+  LopUnkRhs: \<open>\<Delta> \<turnstile> BinOp (unknown[str]: t) (LOp lop) e \<Rrightarrow> unknown[str]: imm\<langle>1\<rangle>\<close> |
+  LopUnkLhs: \<open>\<Delta> \<turnstile> BinOp e (LOp lop) (unknown[str]: t) \<Rrightarrow> unknown[str]: imm\<langle>1\<rangle>\<close> |
+
+  \<comment> \<open>Arithmetic rules\<close>
+  Plus: \<open>\<Delta> \<turnstile> ((num\<^sub>1 \<Colon> sz) + (num\<^sub>2 \<Colon> sz)) \<Rrightarrow> ((num\<^sub>1 \<Colon> sz) +\<^sub>b\<^sub>v (num\<^sub>2 \<Colon> sz))\<close> |
+  Minus: \<open>\<Delta> \<turnstile> ((num\<^sub>1 \<Colon> sz) - (num\<^sub>2 \<Colon> sz)) \<Rrightarrow> ((num\<^sub>1 \<Colon> sz) -\<^sub>b\<^sub>v (num\<^sub>2 \<Colon> sz))\<close> |
+  Times: \<open>\<Delta> \<turnstile> ((num\<^sub>1 \<Colon> sz) * (num\<^sub>2 \<Colon> sz)) \<Rrightarrow> ((num\<^sub>1 \<Colon> sz) *\<^sub>b\<^sub>v (num\<^sub>2 \<Colon> sz))\<close> |
+  Div: \<open>\<Delta> \<turnstile> ((num\<^sub>1 \<Colon> sz) div (num\<^sub>2 \<Colon> sz)) \<Rrightarrow> ((num\<^sub>1 \<Colon> sz) div\<^sub>b\<^sub>v (num\<^sub>2 \<Colon> sz))\<close> |
+  SDiv: \<open>\<Delta> \<turnstile> ((num\<^sub>1 \<Colon> sz) sdiv (num\<^sub>2 \<Colon> sz)) \<Rrightarrow> ((num\<^sub>1 \<Colon> sz) div\<^sub>s\<^sub>b\<^sub>v (num\<^sub>2 \<Colon> sz))\<close> |
+  Mod: \<open>\<Delta> \<turnstile> ((num\<^sub>1 \<Colon> sz) % (num\<^sub>2 \<Colon> sz)) \<Rrightarrow> ((num\<^sub>1 \<Colon> sz) %\<^sub>b\<^sub>v (num\<^sub>2 \<Colon> sz))\<close> |
+  SMod: \<open>\<Delta> \<turnstile> ((num\<^sub>1 \<Colon> sz) smod (num\<^sub>2 \<Colon> sz)) \<Rrightarrow> ((num\<^sub>1 \<Colon> sz) %\<^sub>s\<^sub>b\<^sub>v (num\<^sub>2 \<Colon> sz))\<close> |
+  Lsl: \<open>\<Delta> \<turnstile> ((num\<^sub>1 \<Colon> sz) << (num\<^sub>2 \<Colon> sz)) \<Rrightarrow> ((num\<^sub>1 \<Colon> sz) <<\<^sub>b\<^sub>v (num\<^sub>2 \<Colon> sz))\<close> |
+  Lsr: \<open>\<Delta> \<turnstile> ((num\<^sub>1 \<Colon> sz) >> (num\<^sub>2 \<Colon> sz)) \<Rrightarrow> ((num\<^sub>1 \<Colon> sz) >>\<^sub>b\<^sub>v (num\<^sub>2 \<Colon> sz))\<close> |
+  Asr: \<open>\<Delta> \<turnstile> ((num\<^sub>1 \<Colon> sz) >>> (num\<^sub>2 \<Colon> sz)) \<Rrightarrow> ((num\<^sub>1 \<Colon> sz) >>>\<^sub>b\<^sub>v (num\<^sub>2 \<Colon> sz))\<close> |
+
+  \<comment> \<open>Logical rules\<close>
+  LAnd: \<open>\<Delta> \<turnstile> ((num\<^sub>1 \<Colon> sz) && (num\<^sub>2 \<Colon> sz)) \<Rrightarrow> ((num\<^sub>1 \<Colon> sz) &\<^sub>b\<^sub>v (num\<^sub>2 \<Colon> sz))\<close> |
+  LOr: \<open>\<Delta> \<turnstile> ((num\<^sub>1 \<Colon> sz) || (num\<^sub>2 \<Colon> sz)) \<Rrightarrow> ((num\<^sub>1 \<Colon> sz) |\<^sub>b\<^sub>v (num\<^sub>2 \<Colon> sz))\<close> |
+  XOr: \<open>\<Delta> \<turnstile> ((num\<^sub>1 \<Colon> sz) xor (num\<^sub>2 \<Colon> sz)) \<Rrightarrow> ((num\<^sub>1 \<Colon> sz) xor\<^sub>b\<^sub>v (num\<^sub>2 \<Colon> sz))\<close> |
+  (*these aren't really right*)
+  EqSame: \<open>\<Delta> \<turnstile> (BinOp (num \<Colon> sz) (LOp Eq) (num \<Colon> sz)) \<Rrightarrow> true\<close> |
+  EqDiff: \<open>((num\<^sub>1 \<Colon> sz)::word) \<noteq>\<^sub>b\<^sub>v (num\<^sub>2 \<Colon> sz) = true \<Longrightarrow> \<Delta> \<turnstile> (BinOp (num\<^sub>1 \<Colon> sz) (LOp Eq) (num\<^sub>2 \<Colon> sz)) \<Rrightarrow> false\<close> |
+  NeqSame: \<open>\<Delta> \<turnstile> (BinOp (num \<Colon> sz) (LOp Neq) (num \<Colon> sz)) \<Rrightarrow> false\<close> |
+  NeqDiff: \<open>((num\<^sub>1 \<Colon> sz)::word) \<noteq>\<^sub>b\<^sub>v (num\<^sub>2 \<Colon> sz) = true \<Longrightarrow> \<Delta> \<turnstile> (BinOp (num\<^sub>1 \<Colon> sz)) (LOp Neq) (num\<^sub>2 \<Colon> sz) \<Rrightarrow> true\<close> |
+  Less: \<open>\<Delta> \<turnstile> ((num\<^sub>1 \<Colon> sz) lt (num\<^sub>2 \<Colon> sz)) \<Rrightarrow> ((num\<^sub>1 \<Colon> sz) <\<^sub>b\<^sub>v (num\<^sub>2 \<Colon> sz))\<close> |
+  LessEq: \<open>\<Delta> \<turnstile> ((num\<^sub>1 \<Colon> sz) le (num\<^sub>2 \<Colon> sz)) \<Rrightarrow> ((num\<^sub>1 \<Colon> sz) \<le>\<^sub>b\<^sub>v (num\<^sub>2 \<Colon> sz))\<close> |
+  SignedLess: \<open>\<Delta> \<turnstile> ((num\<^sub>1 \<Colon> sz) slt (num\<^sub>2 \<Colon> sz)) \<Rrightarrow> ((num\<^sub>1 \<Colon> sz) <\<^sub>s\<^sub>b\<^sub>v (num\<^sub>2 \<Colon> sz))\<close> |
+  SignedLessEq: \<open>\<Delta> \<turnstile> ((num\<^sub>1 \<Colon> sz) sle (num\<^sub>2 \<Colon> sz)) \<Rrightarrow> ((num\<^sub>1 \<Colon> sz) \<le>\<^sub>s\<^sub>b\<^sub>v (num\<^sub>2 \<Colon> sz))\<close> |
+
+  \<comment> \<open>Unary op\<close>
+  Uop: \<open>\<Delta> \<turnstile> e \<Rrightarrow> e' \<Longrightarrow> \<Delta> \<turnstile> (UnOp uop e) \<Rrightarrow> (UnOp uop e')\<close> |
+  UopUnk: \<open>\<Delta> \<turnstile> (UnOp uop (unknown[str]: t)) \<Rrightarrow> (unknown[str]: t)\<close> |
+  Not: \<open>\<Delta> \<turnstile> (~(num \<Colon> sz)) \<Rrightarrow> (~\<^sub>b\<^sub>v (num \<Colon> sz))\<close> |
+  Neg: \<open>\<Delta> \<turnstile> (UnOp Neg (num \<Colon> sz)) \<Rrightarrow> (-\<^sub>b\<^sub>v (num \<Colon> sz))\<close> |
+
+  \<comment> \<open>Concat\<close>
+  ConcatRhs: \<open>\<Delta> \<turnstile> e\<^sub>2 \<Rrightarrow> e\<^sub>2' \<Longrightarrow> \<Delta> \<turnstile> (e\<^sub>1 @ e\<^sub>2) \<Rrightarrow> (e\<^sub>1 @ e\<^sub>2')\<close> |
+  ConcatLhs: \<open>\<Delta> \<turnstile> e\<^sub>1 \<Rrightarrow> e\<^sub>1' \<Longrightarrow> \<Delta> \<turnstile> (e\<^sub>1 @ (Val v\<^sub>2)) \<Rrightarrow> (e\<^sub>1' @ (Val v\<^sub>2))\<close> |
+  ConcatRhsUn: \<open>type v = imm\<langle>sz\<^sub>1\<rangle> \<Longrightarrow> \<Delta> \<turnstile> ((Val v) @ (unknown[str]: imm\<langle>sz\<^sub>2\<rangle>)) \<Rrightarrow> (unknown[str]: imm\<langle>sz\<^sub>1 + sz\<^sub>2\<rangle>)\<close> |
+  ConcatLhsUn: \<open>type v = imm\<langle>sz\<^sub>2\<rangle> \<Longrightarrow> \<Delta> \<turnstile> ((unknown[str]: imm\<langle>sz\<^sub>1\<rangle>) @ (Val v)) \<Rrightarrow> (unknown[str]: imm\<langle>sz\<^sub>1 + sz\<^sub>2\<rangle>)\<close> |
+  Concat: \<open>\<Delta> \<turnstile> ((num\<^sub>1 \<Colon> sz\<^sub>1) @ (num\<^sub>2 \<Colon> sz\<^sub>2)) \<Rrightarrow> ((num\<^sub>1 \<Colon> sz\<^sub>1) \<cdot> (num\<^sub>2 \<Colon> sz\<^sub>2))\<close> |
+
+  \<comment> \<open>Extract\<close>
+  Extract: \<open>sz\<^sub>2 \<le> sz\<^sub>1 \<Longrightarrow> \<Delta> \<turnstile> (extract:sz\<^sub>1:sz\<^sub>2[(num \<Colon> sz)]) \<Rrightarrow> (ext (num \<Colon> sz) \<sim> hi : sz\<^sub>1 \<sim> lo : sz\<^sub>2)\<close> |
+  ExtractReduce: \<open>\<Delta> \<turnstile> e \<Rrightarrow> e' \<Longrightarrow> \<Delta> \<turnstile> (extract:sz\<^sub>1:sz\<^sub>2[e]) \<Rrightarrow> (extract:sz\<^sub>1:sz\<^sub>2[e'])\<close> |
+  ExtractUn: \<open>\<Delta> \<turnstile> (extract:sz\<^sub>1:sz\<^sub>2[unknown[str]: t]) \<Rrightarrow> (unknown[str]: imm\<langle>(sz\<^sub>1 - sz\<^sub>2) + 1\<rangle>)\<close> |
+
+  \<comment> \<open>Cast\<close>
+  CastReduce: \<open>\<Delta> \<turnstile> e \<Rrightarrow> e' \<Longrightarrow> \<Delta> \<turnstile> (Cast cast sz e) \<Rrightarrow> (Cast cast sz e')\<close> |
+  CastUnk: \<open>\<Delta> \<turnstile> e \<Rrightarrow> e' \<Longrightarrow> \<Delta> \<turnstile> (Cast cast sz (unknown[str]: t)) \<Rrightarrow> (unknown[str]: imm\<langle>sz\<rangle>)\<close> |
+  CastLow: \<open>\<Delta> \<turnstile> (low:sz[(num \<Colon> sz')]) \<Rrightarrow> (ext (num \<Colon> sz') \<sim> hi : (sz - 1) \<sim> lo : 0)\<close> |
+  CastHigh: \<open>\<Delta> \<turnstile> (high:sz[(num \<Colon> sz')]) \<Rrightarrow> (ext (num \<Colon> sz') \<sim> hi : (sz' - 1) \<sim> lo : (sz' - sz))\<close> |
+  CastSigned: \<open>\<Delta> \<turnstile> (extend:sz[(num \<Colon> sz')]) \<Rrightarrow> (ext (num \<Colon> sz') \<sim> hi : (sz - 1) \<sim> lo : 0)\<close> |
+  CastUnsigned: \<open>\<Delta> \<turnstile> (pad:sz[(num \<Colon> sz')]) \<Rrightarrow> (ext (num \<Colon> sz') \<sim> hi : (sz - 1) \<sim> lo : 0)\<close>
+
+inductive_cases VarE: \<open>\<Delta> \<turnstile> (name' :\<^sub>t t) \<Rrightarrow> e\<close>
+
+inductive_cases LoadStepAddrE: \<open>\<Delta> \<turnstile> e\<^sub>1[e\<^sub>2, ed]:usz \<Rrightarrow> e\<close>
+inductive_cases LoadStepMemE: \<open>\<Delta> \<turnstile> e\<^sub>1[Val v\<^sub>2, ed]:usz \<Rrightarrow> e\<close>
+inductive_cases LoadByteE: \<open>\<Delta> \<turnstile> v[(num \<Colon> sz\<^sub>a\<^sub>d\<^sub>d\<^sub>r) \<leftarrow> v', sz][(num \<Colon> sz\<^sub>a\<^sub>d\<^sub>d\<^sub>r), ed]:usz \<Rrightarrow> e\<close> 
+inductive_cases LoadByteFromNextE: \<open>\<Delta> \<turnstile> ((v[(num\<^sub>1 \<Colon> sz\<^sub>1) \<leftarrow> v', sz][(num\<^sub>2 \<Colon> sz\<^sub>2), ed]:usz)::exp) \<Rrightarrow> e\<close>
+inductive_cases LoadUnMemE: \<open>\<Delta> \<turnstile> (unknown[str]: t)[Val v, ed]:usz \<Rrightarrow> e\<close> 
+inductive_cases LoadUnAddrE: \<open>\<Delta> \<turnstile> v[w \<leftarrow> v', sz][unknown[str]: t, ed]:usz' \<Rrightarrow> e\<close> 
+inductive_cases LoadWordBeE: \<open>\<Delta> \<turnstile> ((Val v)[(num \<Colon> sz\<^sub>a\<^sub>d\<^sub>d\<^sub>r), be]:usz) \<Rrightarrow> e\<close>
+inductive_cases LoadWordElE: \<open>\<Delta> \<turnstile> ((Val v)[(num \<Colon> sz\<^sub>a\<^sub>d\<^sub>d\<^sub>r), el]:usz) \<Rrightarrow> e\<close>
+
+inductive_cases StoreStepValE: \<open>\<Delta> \<turnstile> (e\<^sub>1 with [e\<^sub>2, en]:usz \<leftarrow> e\<^sub>3) \<Rrightarrow> e\<close>
+inductive_cases StoreStepAddrE: \<open>\<Delta> \<turnstile> (e\<^sub>1 with [e\<^sub>2, en]:usz \<leftarrow> (Val v\<^sub>3)) \<Rrightarrow> e\<close>
+inductive_cases StoreStepMemE: \<open>\<Delta> \<turnstile> (e\<^sub>1 with [(Val v\<^sub>2), en]:usz \<leftarrow> (Val v\<^sub>3)) \<Rrightarrow> e\<close>
+inductive_cases StoreWordBeE: \<open>\<Delta> \<turnstile> ((Val v) with [(num \<Colon> sz\<^sub>a\<^sub>d\<^sub>d\<^sub>r), be]:usz \<leftarrow> (Val val)) \<Rrightarrow> e\<close>
+inductive_cases StoreWordElE: \<open>\<Delta> \<turnstile> ((Val v) with [(num \<Colon> sz\<^sub>a\<^sub>d\<^sub>d\<^sub>r), el]:usz \<leftarrow> (Val val)) \<Rrightarrow> e\<close>
+inductive_cases StoreValE: \<open>\<Delta> \<turnstile> ((Val v) with [(num \<Colon> sz\<^sub>a\<^sub>d\<^sub>d\<^sub>r), ed]:usz\<^sub>m\<^sub>e\<^sub>m \<leftarrow> (Val v')) \<Rrightarrow> e\<close>
+inductive_cases StoreUnAddrE: \<open>\<Delta> \<turnstile> ((Val v) with [unknown[str]: imm\<langle>sz\<^sub>a\<^sub>d\<^sub>d\<^sub>r\<rangle>, ed]:usz' \<leftarrow> (Val v')) \<Rrightarrow> e\<close>
+
+inductive_cases IfStepCondE: \<open>\<Delta> \<turnstile> (ite e\<^sub>1 (Val v\<^sub>2) (Val v\<^sub>3)) \<Rrightarrow> e\<close>
+inductive_cases IfStepThenE: \<open>\<Delta> \<turnstile> (ite e\<^sub>1 e\<^sub>2 (Val v\<^sub>3)) \<Rrightarrow> e\<close>
+inductive_cases IfStepElseE: \<open>\<Delta> \<turnstile> (ite e\<^sub>1 e\<^sub>2 e\<^sub>3) \<Rrightarrow> e\<close>
+inductive_cases IfTrueE: \<open>\<Delta> \<turnstile> (ite true (Val v\<^sub>2) (Val v\<^sub>3)) \<Rrightarrow> e\<close>
+inductive_cases IfFalseE: \<open>\<Delta> \<turnstile> (ite false (Val v\<^sub>2) (Val v\<^sub>3)) \<Rrightarrow> e\<close>
+inductive_cases IfUnknownE: \<open>\<Delta> \<turnstile> (ite unknown[str]: t (Val v\<^sub>2) (Val v\<^sub>3)) \<Rrightarrow> e\<close>
+inductive_cases LetStepE: \<open>\<Delta> \<turnstile> (Let var e\<^sub>1 e\<^sub>2) \<Rrightarrow> e\<close>
+inductive_cases BopRhsE: \<open>\<Delta> \<turnstile> BinOp (Val v) bop e\<^sub>2 \<Rrightarrow> e\<close>
+inductive_cases BopLhsE: \<open>\<Delta> \<turnstile> BinOp e\<^sub>1 bop e\<^sub>2 \<Rrightarrow> e\<close>
+inductive_cases AOpE: \<open>\<Delta> \<turnstile> (BinOp e\<^sub>1 (AOp aop) e\<^sub>2) \<Rrightarrow> e'\<close>
+
+inductive_cases PlusE: \<open>\<Delta> \<turnstile> ((num\<^sub>1 \<Colon> sz) + (num\<^sub>2 \<Colon> sz)) \<Rrightarrow> e\<close>
+inductive_cases MinusE: \<open>\<Delta> \<turnstile> ((num\<^sub>1 \<Colon> sz) - (num\<^sub>2 \<Colon> sz)) \<Rrightarrow> e\<close>
+inductive_cases TimesE: \<open>\<Delta> \<turnstile> ((num\<^sub>1 \<Colon> sz) * (num\<^sub>2 \<Colon> sz)) \<Rrightarrow> e\<close>
+inductive_cases DivE: \<open>\<Delta> \<turnstile> ((num\<^sub>1 \<Colon> sz) div (num\<^sub>2 \<Colon> sz)) \<Rrightarrow> e\<close>
+inductive_cases SDivE: \<open>\<Delta> \<turnstile> ((num\<^sub>1 \<Colon> sz) sdiv (num\<^sub>2 \<Colon> sz)) \<Rrightarrow> e\<close>
+inductive_cases ModE: \<open>\<Delta> \<turnstile> ((num\<^sub>1 \<Colon> sz) % (num\<^sub>2 \<Colon> sz)) \<Rrightarrow> e\<close>
+inductive_cases SModE: \<open>\<Delta> \<turnstile> ((num\<^sub>1 \<Colon> sz) smod (num\<^sub>2 \<Colon> sz)) \<Rrightarrow> e\<close>
+inductive_cases LslE: \<open>\<Delta> \<turnstile> ((num\<^sub>1 \<Colon> sz) << (num\<^sub>2 \<Colon> sz)) \<Rrightarrow> e\<close>
+inductive_cases LsrE: \<open>\<Delta> \<turnstile> ((num\<^sub>1 \<Colon> sz) >> (num\<^sub>2 \<Colon> sz)) \<Rrightarrow> e\<close>
+inductive_cases AsrE: \<open>\<Delta> \<turnstile> ((num\<^sub>1 \<Colon> sz) >>> (num\<^sub>2 \<Colon> sz)) \<Rrightarrow> e\<close>
+inductive_cases LAndE: \<open>\<Delta> \<turnstile> ((num\<^sub>1 \<Colon> sz) && (num\<^sub>2 \<Colon> sz)) \<Rrightarrow> e\<close>
+inductive_cases LOrE: \<open>\<Delta> \<turnstile> ((num\<^sub>1 \<Colon> sz) || (num\<^sub>2 \<Colon> sz)) \<Rrightarrow> e\<close>
+inductive_cases XOrE: \<open>\<Delta> \<turnstile> ((num\<^sub>1 \<Colon> sz) xor (num\<^sub>2 \<Colon> sz)) \<Rrightarrow> e\<close>
+inductive_cases EqSameE: \<open>\<Delta> \<turnstile> (BinOp (num \<Colon> sz) (LOp Eq) (num \<Colon> sz)) \<Rrightarrow> e\<close>
+inductive_cases EqDiffE: \<open>\<Delta> \<turnstile> (BinOp (num\<^sub>1 \<Colon> sz) (LOp Eq) (num\<^sub>2 \<Colon> sz)) \<Rrightarrow> e\<close>
+inductive_cases NeqSameE: \<open>\<Delta> \<turnstile> (BinOp (num \<Colon> sz) (LOp Neq) (num \<Colon> sz)) \<Rrightarrow> e\<close>
+inductive_cases NeqDiffE: \<open>\<Delta> \<turnstile> (BinOp (num\<^sub>1 \<Colon> sz)) (LOp Neq) (num\<^sub>2 \<Colon> sz) \<Rrightarrow> e\<close>
+inductive_cases LessE: \<open>\<Delta> \<turnstile> ((num\<^sub>1 \<Colon> sz) lt (num\<^sub>2 \<Colon> sz)) \<Rrightarrow> e\<close>
+inductive_cases LessEqE: \<open>\<Delta> \<turnstile> ((num\<^sub>1 \<Colon> sz) le (num\<^sub>2 \<Colon> sz)) \<Rrightarrow> e\<close>
+inductive_cases SignedLessE: \<open>\<Delta> \<turnstile> ((num\<^sub>1 \<Colon> sz) slt (num\<^sub>2 \<Colon> sz)) \<Rrightarrow> e\<close>
+inductive_cases SignedLessEqE: \<open>\<Delta> \<turnstile> ((num\<^sub>1 \<Colon> sz) sle (num\<^sub>2 \<Colon> sz)) \<Rrightarrow> e\<close>
+inductive_cases UopE: \<open>\<Delta> \<turnstile> (UnOp uop e) \<Rrightarrow> e'\<close>
+inductive_cases UopUnkE: \<open>\<Delta> \<turnstile> (UnOp uop (unknown[str]: t)) \<Rrightarrow> e\<close>
+inductive_cases NotE: \<open>\<Delta> \<turnstile> (~(num \<Colon> sz)) \<Rrightarrow> e\<close>
+inductive_cases NegE: \<open>\<Delta> \<turnstile> (UnOp Neg (num \<Colon> sz)) \<Rrightarrow> e\<close>
+inductive_cases ConcatRhsE: \<open>\<Delta> \<turnstile> (e\<^sub>1 @ e\<^sub>2) \<Rrightarrow> e\<close>
+inductive_cases ConcatLhsE: \<open>\<Delta> \<turnstile> (e\<^sub>1 @ (Val v\<^sub>2)) \<Rrightarrow> e\<close>
+inductive_cases ConcatRhsUnE: \<open>\<Delta> \<turnstile> ((Val v) @ (unknown[str]: imm\<langle>sz\<^sub>2\<rangle>)) \<Rrightarrow> e\<close>
+inductive_cases ConcatLhsUnE: \<open>\<Delta> \<turnstile> ((unknown[str]: imm\<langle>sz\<^sub>1\<rangle>) @ (Val v)) \<Rrightarrow> e\<close>
+inductive_cases ConcatE: \<open>\<Delta> \<turnstile> ((num\<^sub>1 \<Colon> sz\<^sub>1) @ (num\<^sub>2 \<Colon> sz\<^sub>2)) \<Rrightarrow> e\<close>
+inductive_cases ExtractE: \<open>\<Delta> \<turnstile> (extract:sz\<^sub>1:sz\<^sub>2[(num \<Colon> sz)]) \<Rrightarrow> e\<close>
+inductive_cases ExtractReduceE: \<open>\<Delta> \<turnstile> (extract:sz\<^sub>1:sz\<^sub>2[e]) \<Rrightarrow> e'\<close>
+inductive_cases ExtractUnE: \<open>\<Delta> \<turnstile> (extract:sz\<^sub>1:sz\<^sub>2[unknown[str]: t]) \<Rrightarrow> e\<close>
+inductive_cases CastReduceE: \<open>\<Delta> \<turnstile> (Cast cast sz e) \<Rrightarrow> e'\<close>
+inductive_cases CastUnkE: \<open>\<Delta> \<turnstile> (Cast cast sz (unknown[str]: t)) \<Rrightarrow> e\<close>
+inductive_cases CastLowE: \<open>\<Delta> \<turnstile> (low:sz[(num \<Colon> sz')]) \<Rrightarrow> e\<close>
+inductive_cases CastHighE: \<open>\<Delta> \<turnstile> (high:sz[(num \<Colon> sz')]) \<Rrightarrow> e\<close>
+inductive_cases CastSignedE: \<open>\<Delta> \<turnstile> (extend:sz[(num \<Colon> sz')]) \<Rrightarrow> e\<close>
+inductive_cases CastUnsignedE: \<open>\<Delta> \<turnstile> (pad:sz[(num \<Colon> sz')]) \<Rrightarrow> e\<close>
+
+lemma Val_not_inject: "v \<noteq> v' \<Longrightarrow> Val v \<noteq> Val v'"
+  by simp
+
+lemma storage_not_nested_val[intro]: \<open>v[num\<^sub>1 \<Colon> sz\<^sub>1 \<leftarrow> v', sz] \<noteq> v\<close>
+  unfolding storage_constructor_val_def by simp
+
+lemma storage_not_val[simp]: \<open>v[num\<^sub>1 \<Colon> sz\<^sub>1 \<leftarrow> v', sz] \<noteq> Val v\<close>
+  unfolding storage_constructor_exp_def
+  apply (rule Val_not_inject)
+  by (rule storage_not_nested_val)
+
+lemma step_exp_neq': \<open>\<Delta> \<turnstile> e \<Rrightarrow> e' \<Longrightarrow> e \<noteq> e'\<close>
+proof (induct rule: eval_exp'.induct)
+  case (VarIn name' t val \<Delta>)
+  then show ?case 
+    using var.not_val by blast
 next
-  case (VarNotIn name' t str)
-  then show ?thesis sorry
+  case (VarNotIn name' t \<Delta> str)
+  then show ?case by simp
 next
-  case (LoadStepAddr e\<^sub>2 e\<^sub>2' e\<^sub>1 ed sz)
-  then show ?thesis sorry
+  case (Plus \<Delta> num\<^sub>1 sz num\<^sub>2)
+  then show ?case 
+    unfolding plus_exp.simps bv_plus.simps by simp
 next
-  case (LoadStepMem e\<^sub>1 e\<^sub>1' v\<^sub>2 ed sz)
-  then show ?thesis sorry
-qed
-  case (VarIn name' t val)
-  thus ?thesis 
-    using assms(2) unfolding var_eq apply clarify
-    using in_vars_the_simp by blast (* TODO deterministic in_vars*)
+  case (LessEq \<Delta> num\<^sub>1 sz num\<^sub>2)
+  then show ?case 
+    unfolding bv_eq_def by simp
 next
-  case (VarNotIn name' t str)
-  thus ?thesis 
-    using assms(2) val_var_in_vars.simps by auto
+  case (SignedLessEq \<Delta> num\<^sub>1 sz num\<^sub>2)
+  then show ?case 
+    unfolding bv_eq_def by simp
+next
+  case (Extract sz\<^sub>2 sz\<^sub>1 \<Delta> num sz)
+  then show ?case
+    unfolding xtract.simps by simp
+next
+  case (CastLow \<Delta> sz num sz')
+  then show ?case 
+    unfolding xtract.simps by simp
+next
+  case (CastHigh \<Delta> sz num sz')
+  then show ?case 
+    unfolding xtract.simps by simp
+next
+  case (CastSigned \<Delta> sz num sz')
+  then show ?case 
+    unfolding xtract.simps by simp
+next
+  case (CastUnsigned \<Delta> sz num sz')
+  then show ?case 
+    unfolding xtract.simps by simp
 qed simp_all
 
-lemma step_exp_var_not_inE:
-  assumes \<open>\<Delta> \<turnstile> (name' :\<^sub>t t) \<Rrightarrow> e'\<close>
-      and \<open>((name' :\<^sub>t t)) \<notin> dom \<Delta>\<close>
-    shows \<open>\<exists>str. e' = unknown[str]: t\<close>
-using assms(1) proof (cases rule: eval_exp'.cases)
-  case (VarIn name' t val)
-  thus ?thesis 
-    using assms(2) by (simp add: val_var_in_vars.simps) (* TODO *)
-next
-  case (VarNotIn name' t str)
-  thus ?thesis 
-    by simp
-qed simp_all
+lemma step_exp_neq: \<open>\<not>(\<Delta> \<turnstile> e \<Rrightarrow> e)\<close>
+  using step_exp_neq' by auto
 
-lemma step_exp_load_step_addrE:
-  assumes \<open>\<Delta> \<turnstile> e\<^sub>1[e\<^sub>2, ed]:usz \<Rrightarrow> e'\<close>
-    shows \<open>\<Delta> \<turnstile> e\<^sub>2 \<Rrightarrow> e\<^sub>2' \<and> e\<^sub>2 \<noteq> e\<^sub>2'\<close>
-using assms(1) by (cases rule: eval_exp'.cases, simp_all)
+lemma eval_exp'_val_no_step_intermediary: \<open>\<Delta> \<turnstile> e \<Rrightarrow> e' \<Longrightarrow> e \<noteq> (Val v)\<close>
+  by (induct rule: eval_exp'.induct, simp_all)
+
+lemma step_exp_not_val[simp]: \<open>\<not>(\<Delta> \<turnstile> (Val v) \<Rrightarrow> e)\<close>
+  using eval_exp'_val_no_step_intermediary by blast
+
+lemma step_exp_not_word[simp]: \<open>\<not>(\<Delta> \<turnstile> (num \<Colon> sz) \<Rrightarrow> e)\<close>
+  unfolding word_constructor_exp_def by (rule step_exp_not_val)
+
+lemma step_exp_not_unknown[simp]: \<open>\<not>(\<Delta> \<turnstile> (unknown[str]: t) \<Rrightarrow> e)\<close>
+  unfolding unknown_constructor_exp_def by (rule step_exp_not_val)
+
+lemma step_exp_not_true[simp]: \<open>\<not>(\<Delta> \<turnstile> true \<Rrightarrow> e)\<close>
+  unfolding true_exp_def by (rule step_exp_not_val)
+
+lemma step_exp_not_false[simp]: \<open>\<not>(\<Delta> \<turnstile> false \<Rrightarrow> e)\<close>
+  unfolding false_exp_def by (rule step_exp_not_val)
+
+lemma step_exp_not_storage[simp]: \<open>\<not>(\<Delta> \<turnstile> v[w \<leftarrow> v', sz] \<Rrightarrow> e')\<close>
+  unfolding storage_constructor_exp_def by (rule step_exp_not_val)
+
+
+text \<open>We describe a well formed delta as one which\<close>
+
+definition
+  wf\<Delta> :: \<open>variables \<Rightarrow> bool\<close>
+where
+  \<open>wf\<Delta> \<Delta> = (\<forall>var \<in> dom \<Delta>. var_type var = type (the (\<Delta> var)))\<close>
+
+
+function
+  no_unknowns :: \<open>variables \<Rightarrow> exp \<Rightarrow> bool\<close>
+where
+  \<open>no_unknowns _ (unknown[_]: _) = False\<close> |
+  \<open>no_unknowns _ (_ \<Colon> _) = True\<close> |
+  \<open>no_unknowns _ (_[_ \<leftarrow> _, _]) = True\<close> |
+  \<open>no_unknowns \<Delta> (name' :\<^sub>t t) = ((name' :\<^sub>t t) \<in> dom \<Delta> \<and> (\<forall>str t. the (\<Delta> (name' :\<^sub>t t)) \<noteq> unknown[str]: t))\<close> |
+  \<open>no_unknowns \<Delta> (e\<^sub>1[e\<^sub>2, _]:u_) = (no_unknowns \<Delta> e\<^sub>1 \<and> no_unknowns \<Delta> e\<^sub>2)\<close> |
+  \<open>no_unknowns \<Delta> (e\<^sub>1 with [e\<^sub>2, _]:u_ \<leftarrow> e\<^sub>3) = (no_unknowns \<Delta> e\<^sub>1 \<and> no_unknowns \<Delta> e\<^sub>2 \<and> no_unknowns \<Delta> e\<^sub>3)\<close> |
+  \<open>no_unknowns \<Delta> (BinOp e\<^sub>1 _ e\<^sub>2) = (no_unknowns \<Delta> e\<^sub>1 \<and> no_unknowns \<Delta> e\<^sub>2)\<close> |
+  \<open>no_unknowns \<Delta> (UnOp _ e) = (no_unknowns \<Delta> e)\<close> |
+  \<open>no_unknowns \<Delta> (Cast _ _ e) = (no_unknowns \<Delta> e)\<close> |
+  \<open>no_unknowns \<Delta> (Let _ e\<^sub>1 e\<^sub>2) = (no_unknowns \<Delta> e\<^sub>1 \<and> no_unknowns \<Delta> e\<^sub>2)\<close> |
+  \<open>no_unknowns \<Delta> (Ite e\<^sub>1 e\<^sub>2 e\<^sub>3) = (no_unknowns \<Delta> e\<^sub>1 \<and> no_unknowns \<Delta> e\<^sub>2 \<and> no_unknowns \<Delta> e\<^sub>3)\<close> |
+  \<open>no_unknowns \<Delta> (extract:_:_[e]) = (no_unknowns \<Delta> e)\<close> |
+  \<open>no_unknowns \<Delta> (e\<^sub>1 @ e\<^sub>2) = (no_unknowns \<Delta> e\<^sub>1 \<and> no_unknowns \<Delta> e\<^sub>2)\<close>
+  subgoal for P x
+    apply (cases x, simp)
+    subgoal for \<Delta> e
+      by (cases e rule: exp_exhaust, auto)
+    .
+  apply auto
+  apply (metis var_not_unknown_neq)
+  apply (metis concat_not_unknown_neq)
+  apply (metis var_not_word_neq)
+  apply (metis var_not_word_neq)
+  apply (metis concat_not_word_neq)
+  apply (metis concat_not_word_neq)
+  apply (metis var_not_storage_neq)
+  apply (metis var_not_storage_neq)
+  apply (metis concat_not_storage_neq)+
+  done
+termination 
+  apply standard
+  apply (relation \<open>(\<lambda>p. size_class.size (snd p)) <*mlex*> {}\<close>)
+  apply (rule wf_mlex, blast)
+  unfolding append_exp_def
+  by (rule mlex_less, force)+
+
+lemma no_unknowns_ext[simp]: \<open>no_unknowns \<Delta> (ext (num \<Colon> sz) \<sim> hi : sz\<^sub>h\<^sub>i \<sim> lo : sz\<^sub>l\<^sub>o\<^sub>w)\<close>
+  unfolding xtract.simps by simp
+
+lemma no_unknowns_succ[simp]: \<open>no_unknowns \<Delta> (succ (num \<Colon> sz\<^sub>a\<^sub>d\<^sub>d\<^sub>r))\<close>
+  unfolding succ.simps by simp
+
+lemma no_unknowns_true[simp]: \<open>no_unknowns \<Delta> true\<close>
+  by (simp add: true_word)
+
+lemma no_unknowns_false[simp]: \<open>no_unknowns \<Delta> false\<close>
+  by (simp add: false_word)
+
+lemma no_unknowns_Val[intro]: \<open>\<forall>str t. val \<noteq> unknown[str]: t \<Longrightarrow> no_unknowns \<Delta> (Val val)\<close>
+  apply (cases val rule: val_exhaust)
+  apply auto
+  unfolding Val_simp_word Val_simp_storage by simp_all
+
+lemma step_exp_no_unknowns:
+  assumes \<open>\<Delta> \<turnstile> e \<Rrightarrow> e'\<close> and \<open>wf\<Delta> \<Delta>\<close> and \<open>no_unknowns \<Delta> e\<close>
+    shows \<open>no_unknowns \<Delta> e'\<close>
+using assms proof (induction rule: eval_exp'.induct)
+  case (VarIn name' t val \<Delta>)
+  then show ?case 
+    apply auto
+    apply (rule no_unknowns_Val)
+    apply auto
+    subgoal for y str t'
+      apply (erule allE[of _ str], erule allE[of _ t])
+      unfolding val_var_in_vars.simps wf\<Delta>_def 
+      by (metis val_syntax_class.type_unknownI var.sel(2) var_constructor_var_def)
+    .
+next
+  case (LoadByte \<Delta> v num sz\<^sub>a\<^sub>d\<^sub>d\<^sub>r v' sz ed)
+  then show ?case 
+    apply auto
+    sorry
+next
+  case (LoadByteFromNext num\<^sub>1 sz\<^sub>1 num\<^sub>2 sz\<^sub>2 \<Delta> v v' sz ed)
+  then show ?case 
+    apply auto
+    sorry
+next
+  case (LessEq \<Delta> num\<^sub>1 sz num\<^sub>2)
+  then show ?case 
+    unfolding bv_eq_def by auto
+next
+  case (SignedLess \<Delta> num\<^sub>1 sz num\<^sub>2)
+  then show ?case 
+    unfolding bv_le.simps bv_land.simps bv_eq_def by auto
+next
+  case (SignedLessEq \<Delta> num\<^sub>1 sz num\<^sub>2)
+  then show ?case 
+    unfolding bv_le.simps bv_land.simps bv_eq_def by auto
+qed (unfold no_unknowns.simps, simp_all)
 
 
 lemma eval_exp'_deterministic:
   assumes \<open>\<Delta> \<turnstile> e \<Rrightarrow> e\<^sub>1\<close> and \<open>\<Delta> \<turnstile> e \<Rrightarrow> e\<^sub>2\<close>
     shows \<open>e\<^sub>1 = e\<^sub>2\<close>
-  using assms proof (induct rule: eval_exp'.induct)
+using assms proof (induction arbitrary: e\<^sub>2 rule: eval_exp'.induct)
   case (VarIn name' t val \<Delta>)
-  thus ?case by (rule step_exp_var_inE[symmetric, rotated]) 
+  show ?case 
+    using VarIn(2) apply (rule VarE, simp_all)
+    using VarIn.hyps apply (rule var_in_deterministic, blast)
+    using VarIn.hyps val_var_in_vars.simps by blast
 next
   case (VarNotIn name' t \<Delta> str)
-  thus ?case sorry
+  show ?case 
+    using VarNotIn(2) apply (rule VarE, simp_all)
+    using VarNotIn.hyps apply (simp add: val_var_in_vars.simps)
+    subgoal sorry
+    .
 next
-  case (LoadStepAddr \<Delta> e\<^sub>a e\<^sub>a' e\<^sub>m ed sz)
-  thus ?case 
-    using step_exp_load_step_addrE
-    sorry
+  case (LoadStepAddr \<Delta> e\<^sub>2' e\<^sub>2'' e\<^sub>1 ed sz)
+  show ?case 
+    using LoadStepAddr(4) apply (rule LoadStepAddrE)
+    using LoadStepAddr.hyps apply auto
+    by (rule LoadStepAddr.IH)
 next
   case (LoadStepMem \<Delta> e\<^sub>1 e\<^sub>1' v\<^sub>2 ed sz)
-  thus ?case 
-    
+  show ?case 
+    using LoadStepMem(4) apply (rule LoadStepMemE)
+    using LoadStepMem.hyps apply auto
+    by (rule LoadStepMem.IH)
+next
+  case (LoadByte \<Delta> v num sz\<^sub>a\<^sub>d\<^sub>d\<^sub>r v' sz ed)
+  then show ?case 
+    apply (rule LoadByteE, auto)
+    apply (simp_all add: storage_constructor_exp_def)
+    by fastforce+
+next
+  case (LoadByteFromNext num\<^sub>1 sz\<^sub>1 num\<^sub>2 sz\<^sub>2 \<Delta> v v' sz ed)
+  show ?case 
+    using LoadByteFromNext(2) apply (rule LoadByteFromNextE)
+    using LoadByteFromNext.hyps apply auto
+    apply (simp_all add: storage_constructor_exp_def)
+    by fastforce+
+next
+  case (LoadUnMem \<Delta> str t v ed sz)
+  then show ?case 
+    apply (rule LoadUnMemE)
+    apply auto
     sorry
+next
+  case (LoadUnAddr \<Delta> v w v' sz str t ed sz')
+  then show ?case 
+    apply (rule LoadUnAddrE)
+    by auto
+next
+  case (LoadWordBe sz sz\<^sub>m\<^sub>e\<^sub>m v sz\<^sub>a\<^sub>d\<^sub>d\<^sub>r \<Delta> num)
+  show ?case 
+    using LoadWordBe(3) apply (rule LoadWordBeE)
+    using LoadWordBe.hyps apply auto
+    apply (simp_all add: storage_constructor_exp_def)
+    sorry
+next
+  case (LoadWordEl sz sz\<^sub>m\<^sub>e\<^sub>m v sz\<^sub>a\<^sub>d\<^sub>d\<^sub>r \<Delta> num)
+  show ?case 
+    using LoadWordEl(3) apply (rule LoadWordElE)
+    using LoadWordEl.hyps apply auto
+    apply (simp_all add: storage_constructor_exp_def)
+    sorry
+next
+  case (StoreStepVal \<Delta> e\<^sub>3 e\<^sub>3' e\<^sub>1 e\<^sub>2 en sz)
+  show ?case 
+    using StoreStepVal(3) apply (rule StoreStepValE)
+    using StoreStepVal.hyps apply auto
+    by (rule StoreStepVal.IH) 
+next
+  case (StoreStepAddr \<Delta> e\<^sub>2 e\<^sub>2' e\<^sub>1 en sz v\<^sub>3)
+  show ?case 
+    using StoreStepAddr(3) apply (rule StoreStepAddrE)
+    using StoreStepAddr.hyps apply auto
+    by (rule StoreStepAddr.IH) 
+next
+  case (StoreStepMem \<Delta> e\<^sub>1 e\<^sub>1' v\<^sub>2 en sz v\<^sub>3)
+  show ?case 
+    using StoreStepMem(3) apply (rule StoreStepMemE)
+    using StoreStepMem.hyps apply auto
+    by (rule StoreStepMem.IH) 
+next
+  case (StoreWordBe sz\<^sub>m\<^sub>e\<^sub>m sz v sz\<^sub>a\<^sub>d\<^sub>d\<^sub>r e\<^sub>1 num val \<Delta>)
+  show ?case 
+    using StoreWordBe(4) apply (rule StoreWordBeE)
+    using StoreWordBe.hyps by auto
+next
+  case (StoreWordEl sz\<^sub>m\<^sub>e\<^sub>m sz v sz\<^sub>a\<^sub>d\<^sub>d\<^sub>r e\<^sub>1 num val \<Delta>)
+  show ?case 
+    using StoreWordEl(4) apply (rule StoreWordElE)
+    using StoreWordEl.hyps by auto
+next
+  case (StoreVal v sz\<^sub>a\<^sub>d\<^sub>d\<^sub>r sz\<^sub>m\<^sub>e\<^sub>m \<Delta> num ed v')
+  show ?case 
+    using StoreVal(2) apply (rule StoreValE)
+    using StoreVal.hyps by auto
+next
+  case (StoreUnAddr v t \<Delta> str sz\<^sub>a\<^sub>d\<^sub>d\<^sub>r ed sz' v')
+  show ?case 
+    using StoreUnAddr(2) apply (rule StoreUnAddrE)
+    using StoreUnAddr.hyps by auto
+next
+  case (LetStep \<Delta> e\<^sub>1 e\<^sub>1' var e\<^sub>2)
+  show ?case 
+    using LetStep(3) apply (rule LetStepE)
+    using LetStep.hyps apply auto
+    by (rule LetStep.IH) 
+next
+  case (IfStepCond \<Delta> e\<^sub>1 e\<^sub>1' v\<^sub>2 v\<^sub>3)
+  show ?case 
+    using IfStepCond(3) apply (rule IfStepCondE)
+    using IfStepCond.hyps apply auto
+    by (rule IfStepCond.IH) 
+next
+  case (IfStepThen \<Delta> e\<^sub>2 e\<^sub>2' e\<^sub>1 v\<^sub>3)
+  show ?case 
+    using IfStepThen(3) apply (rule IfStepThenE)
+    using IfStepThen.hyps apply auto
+    by (rule IfStepThen.IH) 
+next
+  case (IfStepElse \<Delta> e\<^sub>3 e\<^sub>3' e\<^sub>1 e\<^sub>2)
+  show ?case 
+    using IfStepElse(3) apply (rule IfStepElseE)
+    using IfStepElse.hyps apply auto
+    by (rule IfStepElse.IH) 
+next
+  case (IfTrue \<Delta> v\<^sub>2 v\<^sub>3)
+  then show ?case
+    apply (rule IfTrueE)
+    apply auto
+    using unknown_not_true by metis    
+next
+  case (IfFalse \<Delta> v\<^sub>2 v\<^sub>3)
+  then show ?case 
+    apply (rule IfFalseE)
+    apply auto
+    using unknown_not_false by metis
+next
+  case (IfUnknown v\<^sub>2 t' \<Delta> str t v\<^sub>3)
+  show ?case 
+    using IfUnknown(2) apply (rule IfUnknownE)
+    using IfUnknown.hyps by auto
+next
+  case (BopRhs \<Delta> e\<^sub>2' e\<^sub>2'' v bop)
+  show ?case 
+    using BopRhs(3) apply (rule BopRhsE)
+    using BopRhs.hyps apply auto
+    apply (rule BopRhs.IH, blast)
+    sorry
+next
+  case (BopLhs \<Delta> e\<^sub>1 e\<^sub>1' bop e\<^sub>2')
+  show ?case 
+    using BopLhs(3) apply (rule BopLhsE)
+    using BopLhs.hyps apply auto
+    apply (rule BopLhs.IH, blast)
+    sorry
+next
+  case (AopUnkRhs \<Delta> str t aop e)
+  then show ?case sorry
+next
+  case (AopUnkLhs \<Delta> e aop str t)
+  then show ?case sorry
+next
+  case (LopUnkRhs \<Delta> str t lop e)
+  then show ?case sorry
+next
+  case (LopUnkLhs \<Delta> e lop str t)
+  then show ?case sorry
+next
+  case (Plus \<Delta> num\<^sub>1 sz num\<^sub>2)
+  then show ?case 
+    apply (rule PlusE)
+    by auto
+next
+  case (Minus \<Delta> num\<^sub>1 sz num\<^sub>2)
+  then show ?case 
+    apply (rule MinusE)
+    by auto
+next
+  case (Times \<Delta> num\<^sub>1 sz num\<^sub>2)
+  then show ?case 
+    apply (rule TimesE)
+    by auto
+next
+  case (Div \<Delta> num\<^sub>1 sz num\<^sub>2)
+  then show ?case 
+    apply (rule DivE)
+    by auto
+next
+  case (SDiv \<Delta> num\<^sub>1 sz num\<^sub>2)
+  then show ?case 
+    apply (rule SDivE)
+    by auto
+next
+  case (Mod \<Delta> num\<^sub>1 sz num\<^sub>2)
+  then show ?case 
+    apply (rule ModE)
+    by auto
+next
+  case (SMod \<Delta> num\<^sub>1 sz num\<^sub>2)
+  then show ?case 
+    apply (rule SModE)
+    by auto    
+next
+  case (Lsl \<Delta> num\<^sub>1 sz num\<^sub>2)
+  then show ?case 
+    apply (rule LslE)
+    by auto
+next
+  case (Lsr \<Delta> num\<^sub>1 sz num\<^sub>2)
+  then show ?case 
+    apply (rule LsrE)
+    by auto
+next
+  case (Asr \<Delta> num\<^sub>1 sz num\<^sub>2)
+  then show ?case 
+    apply (rule AsrE)
+    by auto
+next
+  case (LAnd \<Delta> num\<^sub>1 sz num\<^sub>2)
+  then show ?case 
+    apply (rule LAndE)
+    by auto
+next
+  case (LOr \<Delta> num\<^sub>1 sz num\<^sub>2)
+  then show ?case
+    apply (rule LOrE)
+    by auto
+next
+  case (XOr \<Delta> num\<^sub>1 sz num\<^sub>2)
+  then show ?case 
+    apply (rule XOrE)
+    by auto
+next
+  case (EqSame \<Delta> num sz)
+  then show ?case 
+    apply (rule EqSameE)
+    apply auto    
+    by (simp add: bv_eq_def)
+next
+  case (EqDiff num\<^sub>1 sz num\<^sub>2 \<Delta>)
+  show ?case 
+    using EqDiff(2) apply (rule EqDiffE)
+    apply auto
+    by (metis EqDiff.hyps bv_eq_def bv_negation_true_false true_neq_false_word)
+next
+  case (NeqSame \<Delta> num sz)
+  then show ?case 
+    apply (rule NeqSameE)
+    apply auto
+    by (simp add: bv_eq_def)
+next
+  case (NeqDiff num\<^sub>1 sz num\<^sub>2 \<Delta>)
+  show ?case 
+    using NeqDiff(2) apply (rule NeqDiffE)
+    apply auto
+    by (metis NeqDiff.hyps bv_eq_def bv_negation_true_false true_neq_false_word)
+next
+  case (Less \<Delta> num\<^sub>1 sz num\<^sub>2)
+  then show ?case 
+    apply (rule LessE)
+    by auto
+next
+  case (LessEq \<Delta> num\<^sub>1 sz num\<^sub>2)
+  then show ?case 
+    apply (rule LessEqE)
+    by auto
+next
+  case (SignedLess \<Delta> num\<^sub>1 sz num\<^sub>2)
+  then show ?case 
+    apply (rule SignedLessE)
+    by auto
+next
+  case (SignedLessEq \<Delta> num\<^sub>1 sz num\<^sub>2)
+  then show ?case 
+    apply (rule SignedLessEqE)
+    by auto
+next
+  case (Uop \<Delta> e e' uop)
+  show ?case
+    using Uop(3) apply (rule UopE)
+    using Uop.hyps apply auto
+    by (rule Uop.IH) 
+next
+  case (UopUnk \<Delta> uop str t)
+  then show ?case 
+    apply (rule UopUnkE)
+    by auto    
+next
+  case (Not \<Delta> num sz)
+  then show ?case
+    apply (rule NotE)
+    by auto
+next
+  case (Neg \<Delta> num sz)
+  then show ?case 
+    apply (rule NegE)
+    by auto
+next
+  case (ConcatRhs \<Delta> e\<^sub>2 e\<^sub>2' e\<^sub>1)
+  show ?case 
+    using ConcatRhs(3) apply (rule ConcatRhsE)
+    using ConcatRhs.hyps apply auto
+    apply (metis var_not_concat)
+    apply (metis var_not_concat)
+    by (rule ConcatRhs.IH)
+next
+  case (ConcatLhs \<Delta> e\<^sub>1 e\<^sub>1' v\<^sub>2)
+  show ?case 
+    using ConcatLhs(3) apply (rule ConcatLhsE)
+    using ConcatLhs.hyps apply auto
+    apply (metis var_not_concat)
+    apply (metis var_not_concat)
+    by (rule ConcatLhs.IH)
+next
+  case (ConcatRhsUn v sz\<^sub>1 \<Delta> str sz\<^sub>2)
+  show ?case 
+    using ConcatRhsUn(2) apply (rule ConcatRhsUnE)
+    using ConcatRhsUn.hyps apply auto
+    apply (metis var_not_concat)+
+    defer
+    using unknown_constructor_exp_def apply fastforce
+    sorry
+next
+  case (ConcatLhsUn v sz\<^sub>2 \<Delta> str sz\<^sub>1)
+  show ?case 
+    using ConcatLhsUn(2) apply (rule ConcatLhsUnE)
+    using ConcatLhsUn.hyps apply auto
+    apply (metis var_not_concat)+
+    defer
+    using unknown_constructor_exp_def apply fastforce
+    sorry    
+next
+  case (Concat \<Delta> num\<^sub>1 sz\<^sub>1 num\<^sub>2 sz\<^sub>2)
+  then show ?case 
+    apply (rule ConcatE)
+    apply auto
+    apply (metis var_not_concat)
+    by (metis var_not_concat)
+next
+  case (Extract sz\<^sub>2 sz\<^sub>1 \<Delta> num sz)
+  show ?case 
+    using Extract(2) apply (rule ExtractE)
+    using Extract.hyps by auto
+next
+  case (ExtractReduce \<Delta> e e' sz\<^sub>1 sz\<^sub>2)
+  show ?case 
+    using ExtractReduce(3) apply (rule ExtractReduceE)
+    using ExtractReduce.hyps apply auto
+    by (rule ExtractReduce.IH)
+next
+  case (ExtractUn \<Delta> sz\<^sub>1 sz\<^sub>2 str t)
+  then show ?case 
+    apply (rule ExtractUnE)
+    by auto
+next
+  case (CastReduce \<Delta> e e' cast sz)
+  show ?case 
+    using CastReduce(3) apply (rule CastReduceE)
+    using CastReduce.hyps apply auto
+    by (rule CastReduce.IH)
+next
+  case (CastUnk \<Delta> e e' cast sz str t)
+  show ?case 
+    using CastUnk(3) apply (rule CastUnkE)
+    using CastUnk.hyps
+    by auto
+next
+  case (CastLow \<Delta> sz num sz')
+  then show ?case
+    apply (rule CastLowE)
+    by auto
+next
+  case (CastHigh \<Delta> sz num sz')
+  then show ?case 
+    apply (rule CastHighE)
+    by auto
+next
+  case (CastSigned \<Delta> sz num sz')
+  then show ?case 
+    apply (rule CastSignedE)
+    by auto
+next
+  case (CastUnsigned \<Delta> sz num sz')
+  then show ?case 
+    apply (rule CastUnsignedE)
+    by auto
 qed
-*)
+
+
+declare bv_plus.simps[simp del]
+declare plus_exp.simps[simp del]
 
 
 end
