OperationalSemantics/Program_Elims.thy
@@ -9,7 +9,7 @@ begin
 lemma step_progE:
   assumes \<open>(\<Delta>, w\<^sub>1, mem) \<leadsto>\<^sub>b\<^sub>i\<^sub>l (\<Delta>', w\<^sub>3, mem')\<close>
       and \<open>(\<Delta>, w\<^sub>1, mem) \<mapsto>\<^sub>b\<^sub>i\<^sub>l \<lparr> addr = w\<^sub>1, size = w\<^sub>2, code = bil \<rparr>\<close>
-    shows \<open>\<Delta>, (w\<^sub>1 +\<^sub>b\<^sub>v w\<^sub>2) \<turnstile> bil \<leadsto> \<Delta>', w\<^sub>3, Empty\<close>
+    shows \<open>\<Delta>, (w\<^sub>1 +\<^sub>b\<^sub>v w\<^sub>2) \<turnstile> bil \<leadsto> \<Delta>', w\<^sub>3\<close>
 proof (cases \<open>mem = mem'\<close>)
   case True
   then show ?thesis 
