OperationalSemantics/Program_Intros.thy
@@ -8,7 +8,7 @@ begin
 
 lemma step_progI:
   assumes \<open>(\<Delta>, w\<^sub>1, mem) \<mapsto>\<^sub>b\<^sub>i\<^sub>l \<lparr> addr = w\<^sub>1, size = w\<^sub>2, code = bil \<rparr>\<close>
-      and \<open>\<Delta>,w\<^sub>1 +\<^sub>b\<^sub>v w\<^sub>2 \<turnstile> bil \<leadsto> \<Delta>',w',Empty\<close>
+      and \<open>\<Delta>,w\<^sub>1 +\<^sub>b\<^sub>v w\<^sub>2 \<turnstile> bil \<leadsto> \<Delta>',w'\<close>
     shows \<open>(\<Delta>, w\<^sub>1, mem) \<leadsto>\<^sub>b\<^sub>i\<^sub>l (\<Delta>', w', mem)\<close>
   unfolding step_pred.simps
   apply (rule exI[of _ w\<^sub>2])
@@ -20,13 +20,12 @@ lemma step_progI:
 lemma step_prog_noinsnI:
   assumes \<open>(\<Delta>, (num \<Colon> sz), mem) \<mapsto>\<^sub>b\<^sub>i\<^sub>l no_insn (num \<Colon> sz)\<close> and \<open>num < 2 ^ sz\<close>
     shows \<open>(\<Delta>, (num \<Colon> sz), mem) \<leadsto>\<^sub>b\<^sub>i\<^sub>l (\<Delta>, (num \<Colon> sz), mem)\<close>
-  apply (rule step_progI[of _ _ _ \<open>(0 \<Colon> sz)\<close> Empty])
+  apply (rule step_progI[of _ _ _ \<open>(0 \<Colon> sz)\<close> \<open>[]\<close>])
   subgoal 
     using assms(1) by simp
   subgoal
     unfolding bv_plus.simps apply simp
-    using assms(2) apply auto
-    by (rule SEQ_NIL)
+    using assms(2) by auto
   .
 
 end
