StatementSemantics/Statement_Intros.thy
@@ -3,25 +3,60 @@ theory Statement_Intros
           "../ExpressionSemantics/Expression_Intros"
 begin
 
-lemmas step_bil_emptyI = Eq[of _ _ Empty]
-lemmas step_bil_nextI = Next
+lemma step_bil_emptyI[intro!]: \<open>\<Delta>,w \<turnstile> ([]::bil) \<leadsto> \<Delta>,w\<close>
+  unfolding step_syntax_list_def by (rule Empty)
 
-lemma step_bil_seqI:
-  assumes \<open>\<Delta>,w \<turnstile> s\<^sub>1 \<leadsto> \<Delta>',w'\<close>
-    shows \<open>\<Delta>,w \<turnstile> Stmt s\<^sub>1 seq \<leadsto> \<Delta>',w',seq\<close>
-  using assms apply (rule step_bil_nextI)
-  apply (rule Eq)
-  by simp
+lemma step_bil_seqI[intro]:
+  fixes s :: stmt
+  assumes \<open>\<Delta>\<^sub>1,w\<^sub>1 \<turnstile> s \<leadsto> \<Delta>\<^sub>2,w\<^sub>2\<close> and \<open>\<Delta>\<^sub>2,w\<^sub>2 \<turnstile> seq \<leadsto> \<Delta>\<^sub>3,w\<^sub>3\<close>
+    shows \<open>\<Delta>\<^sub>1,w\<^sub>1 \<turnstile> (s # seq) \<leadsto> \<Delta>\<^sub>3,w\<^sub>3\<close>
+  using assms unfolding step_syntax_stmt_def step_syntax_list_def by (rule Next)
 
-lemmas step_stmt_whileI = WhileTrue
-lemmas step_stmt_while_falseI = WhileFalse
-lemmas step_stmt_if_trueI = IfTrue
-lemmas step_stmt_if_then_trueI = step_stmt_if_trueI[of _ _ _ _ _ _ Empty]
-lemmas step_stmt_if_falseI = IfFalse
-lemmas step_stmt_jmpI = Jmp
-lemmas step_stmt_moveI = Move
-lemmas step_stmt_cpuexnI = CpuExn
-lemmas step_stmt_specialI = Special
+lemma step_bil_singleI[intro]:
+  fixes s :: stmt
+  assumes \<open>\<Delta>\<^sub>1,w\<^sub>1 \<turnstile> s \<leadsto> \<Delta>\<^sub>2,w\<^sub>2\<close>
+    shows \<open>\<Delta>\<^sub>1,w\<^sub>1 \<turnstile> [s] \<leadsto> \<Delta>\<^sub>2,w\<^sub>2\<close>
+  using assms apply (rule step_bil_seqI)
+  by (rule step_bil_emptyI)
+
+lemma step_stmt_whileI[intro]:
+  assumes \<open>\<Delta>\<^sub>1 \<turnstile> e \<leadsto>* true\<close> and \<open>\<Delta>\<^sub>1,w\<^sub>1 \<turnstile> seq \<leadsto> \<Delta>\<^sub>2,w\<^sub>2\<close>
+      and \<open>\<Delta>\<^sub>2,w\<^sub>2 \<turnstile> (While e seq) \<leadsto> \<Delta>\<^sub>3,w\<^sub>3\<close>
+    shows \<open>\<Delta>\<^sub>1,w\<^sub>1 \<turnstile> (While e seq) \<leadsto> \<Delta>\<^sub>3,w\<^sub>3\<close>
+  using assms unfolding step_syntax_stmt_def step_syntax_list_def by (rule WhileTrue)
+
+lemma step_stmt_while_falseI[intro]:
+  assumes \<open>\<Delta> \<turnstile> e \<leadsto>* false\<close>
+    shows \<open>\<Delta>,w \<turnstile> (While e seq) \<leadsto> \<Delta>,w\<close>
+  using assms unfolding step_syntax_stmt_def step_syntax_list_def by (rule WhileFalse)
+
+lemma step_stmt_if_trueI[intro]:
+  assumes \<open>\<Delta>\<^sub>1 \<turnstile> e \<leadsto>* true\<close> and \<open>\<Delta>\<^sub>1,w\<^sub>1 \<turnstile> seq\<^sub>1 \<leadsto> \<Delta>\<^sub>2,w\<^sub>2\<close>
+    shows \<open>\<Delta>\<^sub>1,w\<^sub>1 \<turnstile> (If e seq\<^sub>1 seq\<^sub>2) \<leadsto> \<Delta>\<^sub>2,w\<^sub>2\<close>
+  using assms unfolding step_syntax_stmt_def step_syntax_list_def by (rule IfTrue)
+
+lemmas step_stmt_if_then_trueI = step_stmt_if_trueI[of _ _ _ _ _ _ \<open>[]\<close>]
+
+lemma step_stmt_if_falseI:
+  assumes \<open>\<Delta>\<^sub>1 \<turnstile> e \<leadsto>* false\<close> and \<open>\<Delta>\<^sub>1,w\<^sub>1 \<turnstile> seq\<^sub>2 \<leadsto> \<Delta>\<^sub>2,w\<^sub>2\<close>
+    shows \<open>\<Delta>\<^sub>1,w\<^sub>1 \<turnstile> (If e seq\<^sub>1 seq\<^sub>2) \<leadsto> \<Delta>\<^sub>2,w\<^sub>2\<close>
+  using assms unfolding step_syntax_stmt_def step_syntax_list_def by (rule IfFalse)
+
+lemma step_stmt_jmpI:
+  assumes \<open>\<Delta> \<turnstile> e \<leadsto>* (num \<Colon> sz)\<close>
+    shows \<open>\<Delta>,w \<turnstile> jmp e \<leadsto> \<Delta>,(num \<Colon> sz)\<close>
+  using assms unfolding step_syntax_stmt_def step_syntax_list_def by (rule Jmp)
+
+lemma step_stmt_moveI:
+  assumes \<open>\<Delta> \<turnstile> e \<leadsto>* v\<close>
+    shows \<open>\<Delta>,w \<turnstile> (var := e) \<leadsto> (\<Delta>(var \<mapsto> v)),w\<close>
+  using assms unfolding step_syntax_stmt_def step_syntax_list_def by (rule Move)
+
+lemma step_stmt_cpuexnI: "\<Delta>,w \<turnstile> (cpuexn code) \<leadsto> \<Delta>,w"
+   unfolding step_syntax_stmt_def step_syntax_list_def by (rule CpuExn)
+
+lemma step_stmt_specialI: "\<Delta>,w \<turnstile> (special[str]) \<leadsto> \<Delta>,w"
+   unfolding step_syntax_stmt_def step_syntax_list_def by (rule Special)
 
 lemma step_stmt_if_then_falseI:
   assumes \<open>\<Delta> \<turnstile> e \<leadsto>* false\<close>
@@ -29,11 +64,9 @@ lemma step_stmt_if_then_falseI:
   using assms apply (rule step_stmt_if_falseI)
   by (rule step_bil_emptyI)
 
-
+(* Old names  *)
 lemmas SEQ_NIL = step_bil_emptyI
-lemmas SEQ_ONE = step_bil_seqI[of _ _ _ _ _ Empty]
 lemmas SEQ_REC = step_bil_seqI
-lemmas SEQ_LAST = step_bil_seqI[of _ _ _ _ _ \<open>Stmt _ Empty\<close>]
 
 lemmas WHILE = step_stmt_whileI
 lemmas WHILE_FALSE = step_stmt_while_falseI
@@ -45,24 +78,5 @@ lemmas JMP = step_stmt_jmpI
 lemmas MOVE = step_stmt_moveI
 lemmas CPUEXN = step_stmt_cpuexnI
 lemmas SPECIAL = step_stmt_specialI
-
-(*
-lemma SEQ_NIL_NEQ: 
-  assumes \<open>\<Delta>\<noteq>\<Delta>' \<or> w\<noteq>w\<close> 
-    shows \<open>\<not>(\<Delta>',w' \<turnstile> Empty \<leadsto> \<Delta>,w,Empty)\<close>
-  using assms step_pred_bil_def by (metis bil.distinct(1) eval_inf_bil.simps)
-
-lemma SEQ_TOTAL_REC: 
-    \<open>(\<Delta>,w \<turnstile> seq \<leadsto> \<Delta>',w',Empty) \<longleftrightarrow> eval_inf_bil \<Delta> w seq \<Delta>' w'\<close>
-  apply (auto simp add: step_pred_bil_def)
-  apply (simp add: eval_inf_stmt_eval_inf_bil.intros(10))
-  by (metis bil.distinct(1) eval_inf_bil.simps)
-
-lemma SEQ_NEXT:
-  assumes \<open>\<Delta>,w \<turnstile> s\<^sub>1 \<leadsto> \<Delta>',w'\<close> and \<open>\<Delta>',w' \<turnstile> seq \<leadsto> \<Delta>'',w'',Empty\<close>
-    shows \<open>\<Delta>,w \<turnstile> Stmt s\<^sub>1 seq \<leadsto> \<Delta>'',w'',Empty\<close>
-  using assms eval_inf_stmt_eval_inf_bil.intros(9) eval_pred_stmt_def step_pred_bil_empty_equiv by blast
-*)
-
 
 end
