StatementSemantics/Statement_Syntax.thy
@@ -1,7 +1,7 @@
 theory Statement_Syntax
   imports "../ExpressionSemantics/Expression_Syntax"
 begin
-
+(*
 text \<open>If we include a while loop we must use an inductive predicate as the bil/stmt may not 
       terminate ie: while true {}.\<close> 
 
@@ -138,21 +138,61 @@ where
   \<open>\<Delta>,w \<turnstile> s\<^sub>1 \<leadsto> \<Delta>',w' = (eval_inf_stmt \<Delta> w s\<^sub>1 \<Delta>' w')\<close>
 *)
 
+*)
 
 inductive
-  step_pred_stmt :: \<open>variables \<Rightarrow> word \<Rightarrow> stmt \<Rightarrow> variables \<Rightarrow> word \<Rightarrow> bool\<close> (\<open>_,_ \<turnstile> _ \<leadsto> _,_\<close>) and
-  step_pred_bil :: \<open>variables \<Rightarrow> word \<Rightarrow> bil \<Rightarrow> variables \<Rightarrow> word \<Rightarrow> bil \<Rightarrow> bool\<close> (\<open>_,_ \<turnstile> _ \<leadsto> _,_,_\<close>)
+  step_pred_stmt :: \<open>variables \<Rightarrow> word \<Rightarrow> stmt \<Rightarrow> variables \<Rightarrow> word \<Rightarrow> bool\<close> and
+  step_pred_bil :: \<open>variables \<Rightarrow> word \<Rightarrow> bil \<Rightarrow> variables \<Rightarrow> word \<Rightarrow> bool\<close>
 where
-  WhileTrue: \<open>\<lbrakk>\<Delta>\<^sub>1 \<turnstile> e \<leadsto>* true; \<Delta>\<^sub>1,w\<^sub>1 \<turnstile> seq \<leadsto> \<Delta>\<^sub>2, w\<^sub>2, Empty; \<Delta>\<^sub>2,w\<^sub>2 \<turnstile> (While e seq) \<leadsto> \<Delta>\<^sub>3, w\<^sub>3\<rbrakk> \<Longrightarrow> \<Delta>\<^sub>1,w\<^sub>1 \<turnstile> (While e seq) \<leadsto> \<Delta>\<^sub>3, w\<^sub>3\<close> |
-  WhileFalse: \<open>\<lbrakk>\<Delta> \<turnstile> e \<leadsto>* false\<rbrakk> \<Longrightarrow> \<Delta>,w \<turnstile> (While e seq) \<leadsto> \<Delta>,w\<close> |
-  IfTrue: \<open>\<lbrakk>\<Delta> \<turnstile> e \<leadsto>* true; \<Delta>,w \<turnstile> seq\<^sub>1 \<leadsto> \<Delta>',w',Empty\<rbrakk> \<Longrightarrow> \<Delta>,w \<turnstile> (If e seq\<^sub>1 seq\<^sub>2) \<leadsto> \<Delta>', w'\<close> |
-  IfFalse: \<open>\<lbrakk>\<Delta> \<turnstile> e \<leadsto>* false; \<Delta>,w \<turnstile> seq\<^sub>2 \<leadsto> \<Delta>',w',Empty\<rbrakk> \<Longrightarrow> \<Delta>,w \<turnstile> (If e seq\<^sub>1 seq\<^sub>2) \<leadsto> \<Delta>', w'\<close> |
-  Jmp: \<open>\<lbrakk>\<Delta> \<turnstile> e \<leadsto>* (num \<Colon> sz)\<rbrakk> \<Longrightarrow> \<Delta>,w \<turnstile> (Jmp e) \<leadsto> \<Delta>,(num \<Colon> sz)\<close> |
-  Move: \<open>\<lbrakk>\<Delta> \<turnstile> e \<leadsto>* v\<rbrakk> \<Longrightarrow> \<Delta>,w \<turnstile> (Move var e) \<leadsto> \<Delta>(var \<mapsto> v),w\<close> |
-  CpuExn: \<open>\<Delta>,w \<turnstile> (CpuExn code) \<leadsto> \<Delta>,w\<close> |
-  Special: \<open>\<Delta>,w \<turnstile> (Special str) \<leadsto> \<Delta>,w\<close> |
-  Next: \<open>\<lbrakk>\<Delta>,w \<turnstile> s\<^sub>1 \<leadsto> \<Delta>'',w''; \<Delta>'',w'' \<turnstile> seq \<leadsto> \<Delta>',w',seq'; seq' \<noteq> Stmt s\<^sub>1 seq\<rbrakk> \<Longrightarrow> \<Delta>,w \<turnstile> Stmt s\<^sub>1 seq \<leadsto> \<Delta>',w',seq'\<close> |
-  Eq: \<open>\<Delta>,w \<turnstile> seq \<leadsto> \<Delta>,w,seq\<close>
+  WhileTrue: \<open>\<lbrakk>\<Delta>\<^sub>1 \<turnstile> e \<leadsto>* true; step_pred_bil \<Delta>\<^sub>1 w\<^sub>1 seq \<Delta>\<^sub>2 w\<^sub>2; step_pred_stmt \<Delta>\<^sub>2 w\<^sub>2 (While e seq) \<Delta>\<^sub>3 w\<^sub>3\<rbrakk> \<Longrightarrow> step_pred_stmt \<Delta>\<^sub>1 w\<^sub>1  (While e seq) \<Delta>\<^sub>3 w\<^sub>3\<close> |
+  WhileFalse: \<open>\<lbrakk>\<Delta> \<turnstile> e \<leadsto>* false\<rbrakk> \<Longrightarrow> step_pred_stmt \<Delta> w (While e seq) \<Delta> w\<close> |
+  IfTrue: \<open>\<lbrakk>\<Delta> \<turnstile> e \<leadsto>* true; step_pred_bil \<Delta> w seq\<^sub>1 \<Delta>' w'\<rbrakk> \<Longrightarrow> step_pred_stmt \<Delta> w (If e seq\<^sub>1 seq\<^sub>2) \<Delta>' w'\<close> |
+  IfFalse: \<open>\<lbrakk>\<Delta> \<turnstile> e \<leadsto>* false; step_pred_bil \<Delta> w seq\<^sub>2 \<Delta>' w'\<rbrakk> \<Longrightarrow> step_pred_stmt \<Delta> w (If e seq\<^sub>1 seq\<^sub>2) \<Delta>' w'\<close> |
+  Jmp: \<open>\<lbrakk>\<Delta> \<turnstile> e \<leadsto>* (num \<Colon> sz)\<rbrakk> \<Longrightarrow> step_pred_stmt \<Delta> w (Jmp e) \<Delta> (num \<Colon> sz)\<close> |
+  Move: \<open>\<lbrakk>\<Delta> \<turnstile> e \<leadsto>* v\<rbrakk> \<Longrightarrow> step_pred_stmt \<Delta> w (Move var e) (\<Delta>(var \<mapsto> v)) w\<close> |
+  CpuExn: \<open>step_pred_stmt \<Delta> w (CpuExn code) \<Delta> w\<close> |
+  Special: \<open>step_pred_stmt \<Delta> w (Special str) \<Delta> w\<close> |
+  Next: \<open>\<lbrakk>step_pred_stmt \<Delta> w s \<Delta>'' w''; step_pred_bil \<Delta>'' w'' seq \<Delta>' w'\<rbrakk> \<Longrightarrow> step_pred_bil \<Delta> w (s # seq) \<Delta>' w'\<close> |
+  Empty: \<open>step_pred_bil \<Delta> w [] \<Delta> w\<close>
 
+inductive_cases NextE[elim!]: \<open>step_pred_bil \<Delta> w (s # seq) \<Delta>' w'\<close>
+inductive_cases EmptyE[elim!]: \<open>step_pred_bil \<Delta> w [] \<Delta>' w'\<close>
+
+inductive_cases SpecialE[elim!]: \<open>step_pred_stmt \<Delta> w (Special str) \<Delta>' w'\<close>
+inductive_cases CpuExnE[elim!]: \<open>step_pred_stmt \<Delta> w (CpuExn code) \<Delta>' w'\<close>
+inductive_cases MoveE[elim!]: \<open>step_pred_stmt \<Delta> w (Move var e) \<Delta>' w'\<close>
+inductive_cases JmpE[elim!]: \<open>step_pred_stmt \<Delta> w (Jmp e) \<Delta>' w'\<close>
+inductive_cases IfE[elim!]: \<open>step_pred_stmt \<Delta> w (If e seq\<^sub>1 seq\<^sub>2) \<Delta>' w'\<close>
+inductive_cases WhileE[elim]: \<open>step_pred_stmt \<Delta> w (While e seq) \<Delta>' w'\<close>
+
+declare step_pred_stmt_step_pred_bil.intros [intro]
+
+text \<open>Fix syntax for BIL statements classes\<close>
+
+class step_syntax = 
+  fixes step_syntax :: \<open>variables \<Rightarrow> word \<Rightarrow> 'a \<Rightarrow> variables \<Rightarrow> word \<Rightarrow> bool\<close> (\<open>_,_ \<turnstile> _ \<leadsto> _,_\<close>)
+
+instantiation list :: (step_syntax) step_syntax
+begin 
+
+definition
+  step_syntax_list :: \<open>variables \<Rightarrow> word \<Rightarrow> bil \<Rightarrow> variables \<Rightarrow> word \<Rightarrow> bool\<close>
+where
+  \<open>step_syntax_list \<equiv> step_pred_bil\<close>
+
+instance .. 
+end
+
+instantiation stmt :: step_syntax
+begin 
+
+definition
+  step_syntax_stmt :: \<open>variables \<Rightarrow> word \<Rightarrow> stmt \<Rightarrow> variables \<Rightarrow> word \<Rightarrow> bool\<close>
+where
+  \<open>step_syntax_stmt \<equiv> step_pred_stmt\<close>
+
+
+instance .. 
+end
 
 end
