Typing/Typing_BIL_Is_Ok.thy
@@ -1,43 +1,76 @@
 theory Typing_BIL_Is_Ok
   imports Typing_Exp_Typed_Ok
 begin            
-
-class typing_is_ok =
-  fixes typing_is_ok :: \<open>TypingContext \<Rightarrow> 'a \<Rightarrow> bool\<close> (\<open>_ \<turnstile> _ is ok\<close> [260, 235] 201)
-
-instantiation stmt and bil :: typing_is_ok
-begin
-
-function
+(*
+fun
   typing_is_ok_stmt :: \<open>TypingContext \<Rightarrow> stmt \<Rightarrow> bool\<close> and
   typing_is_ok_bil :: \<open>TypingContext \<Rightarrow> bil \<Rightarrow> bool\<close>
 where
-  \<open>typing_is_ok_stmt \<Gamma> (Move (id' :\<^sub>t t) e) = ((\<Gamma> \<turnstile> ((id' :\<^sub>t t)::exp) :: t) \<and> (\<Gamma> \<turnstile> e :: t))\<close> |
+  \<open>typing_is_ok_stmt \<Gamma> (Move (var.Var id' t) e) = ((\<Gamma> \<turnstile> (exp.Var (var.Var id' t)) :: t) \<and> (\<Gamma> \<turnstile> e :: t))\<close> |
   \<open>typing_is_ok_stmt \<Gamma> (Jmp e) = (\<exists>sz. (\<Gamma> \<turnstile> e :: imm\<langle>sz\<rangle>))\<close> |
   \<open>typing_is_ok_stmt \<Gamma> (CpuExn _) = (\<Gamma> is ok)\<close> |
   \<open>typing_is_ok_stmt \<Gamma> (Special _) = (\<Gamma> is ok)\<close> |
-  \<open>typing_is_ok_stmt \<Gamma> (While e seq) = ((\<Gamma> \<turnstile> seq is ok) \<and> (\<Gamma> \<turnstile> e :: imm\<langle>1\<rangle>))\<close> |
-  \<open>typing_is_ok_stmt \<Gamma> (If e seq\<^sub>1 seq\<^sub>2) = ((\<Gamma> \<turnstile> seq\<^sub>1 is ok) \<and> (\<Gamma> \<turnstile> seq\<^sub>2 is ok) \<and> (\<Gamma> \<turnstile> e :: imm\<langle>1\<rangle>))\<close> |
-  \<open>typing_is_ok_bil \<Gamma> Empty = True\<close> |
-  \<open>typing_is_ok_bil \<Gamma> (Stmt stmt seq) = ((\<Gamma> \<turnstile> stmt is ok) \<and> (\<Gamma> \<turnstile> seq is ok))\<close>
+  \<open>typing_is_ok_stmt \<Gamma> (While e seq) = ((typing_is_ok_bil \<Gamma> seq) \<and> (\<Gamma> \<turnstile> e :: imm\<langle>1\<rangle>))\<close> |
+  \<open>typing_is_ok_stmt \<Gamma> (If e seq\<^sub>1 seq\<^sub>2) = ((typing_is_ok_bil \<Gamma> seq\<^sub>1) \<and> (typing_is_ok_bil \<Gamma> seq\<^sub>2) \<and> (\<Gamma> \<turnstile> e :: imm\<langle>1\<rangle>))\<close> |
+  \<open>typing_is_ok_bil \<Gamma> [] = True\<close> |
+  \<open>typing_is_ok_bil \<Gamma> (stmt # seq) = ((typing_is_ok_stmt \<Gamma> stmt) \<and> (typing_is_ok_bil \<Gamma> seq))\<close>
+*)
+
+function
+  typing_is_ok_stmt' :: \<open>TypingContext \<Rightarrow> stmt \<Rightarrow> bool\<close> and
+  typing_is_ok_bil' :: \<open>TypingContext \<Rightarrow> bil \<Rightarrow> bool\<close>
+where
+  \<open>typing_is_ok_stmt' \<Gamma> (Move (id' :\<^sub>t t) e) = ((\<Gamma> \<turnstile> ((id' :\<^sub>t t)::exp) :: t) \<and> (\<Gamma> \<turnstile> e :: t))\<close> |
+  \<open>typing_is_ok_stmt' \<Gamma> (Jmp e) = (\<exists>sz. (\<Gamma> \<turnstile> e :: imm\<langle>sz\<rangle>))\<close> |
+  \<open>typing_is_ok_stmt' \<Gamma> (CpuExn _) = (\<Gamma> is ok)\<close> |
+  \<open>typing_is_ok_stmt' \<Gamma> (Special _) = (\<Gamma> is ok)\<close> |
+  \<open>typing_is_ok_stmt' \<Gamma> (While e seq) = ((typing_is_ok_bil' \<Gamma> seq) \<and> (\<Gamma> \<turnstile> e :: imm\<langle>1\<rangle>))\<close> |
+  \<open>typing_is_ok_stmt' \<Gamma> (If e seq\<^sub>1 seq\<^sub>2) = ((typing_is_ok_bil' \<Gamma> seq\<^sub>1) \<and> (typing_is_ok_bil' \<Gamma> seq\<^sub>2) \<and> (\<Gamma> \<turnstile> e :: imm\<langle>1\<rangle>))\<close> |
+  \<open>typing_is_ok_bil' \<Gamma> [] = True\<close> |
+  \<open>typing_is_ok_bil' \<Gamma> (stmt # seq) = ((typing_is_ok_stmt' \<Gamma> stmt) \<and> (typing_is_ok_bil' \<Gamma> seq))\<close>
   apply simp_all
   subgoal for P x 
     apply (rule obj_sumE[of x])
     apply auto
     subgoal for a b
-      apply (rule stmt.exhaust[of b])
+      apply (cases b rule: stmt.exhaust)
       apply simp_all
       using var_exhaust by auto
     subgoal for a b
-      apply (rule bil.exhaust[of b])
+      apply (cases b)
       by blast+
     .
   .
 termination
   apply standard
-  apply (relation \<open>(case_sum (\<lambda>p. size (snd p)) (\<lambda>p. size (snd p)) <*mlex*> {})\<close>)
+  apply (relation \<open>case_sum (\<lambda>p. size (snd p)) (\<lambda>p. size_list size (snd p)) <*mlex*> {}\<close>)
   apply (rule wf_mlex, blast)
   by (rule mlex_less, simp)+
+
+
+class typing_is_ok =
+  fixes typing_is_ok :: \<open>TypingContext \<Rightarrow> 'a \<Rightarrow> bool\<close> (\<open>_ \<turnstile> _ is ok\<close> [260, 235] 201)
+
+
+instantiation stmt :: typing_is_ok
+begin
+
+definition
+  typing_is_ok_stmt :: \<open>TypingContext \<Rightarrow> stmt \<Rightarrow> bool\<close>
+where
+  \<open>typing_is_ok_stmt \<equiv> typing_is_ok_stmt'\<close>
+
+instance ..
+
+end
+
+instantiation list :: (typing_is_ok) typing_is_ok
+begin
+
+definition
+  typing_is_ok_list :: \<open>TypingContext \<Rightarrow> bil \<Rightarrow> bool\<close>
+where
+  \<open>typing_is_ok_list \<equiv> typing_is_ok_bil'\<close>
 
 instance ..
 
@@ -45,28 +78,32 @@ end
 
 lemma empty_seq_typing_is_ok: 
   assumes \<open>\<Gamma> is ok\<close>
-    shows \<open>\<Gamma> \<turnstile> Empty is ok\<close>
-  by simp
+    shows \<open>\<Gamma> \<turnstile> ([]::bil) is ok\<close>
+  unfolding typing_is_ok_list_def by simp
 
 lemma rec_seq_typing_is_okI: 
+    fixes stmt :: stmt
   assumes \<open>\<Gamma> \<turnstile> stmt is ok\<close> and \<open>\<Gamma> \<turnstile> seq is ok\<close>
-    shows \<open>\<Gamma> \<turnstile> Stmt stmt seq is ok\<close>
-  using assms by auto
+    shows \<open>\<Gamma> \<turnstile> (stmt # seq) is ok\<close>
+  using assms unfolding typing_is_ok_list_def typing_is_ok_stmt_def by auto
 
 lemma rec_seq_typing_is_okE: 
-  assumes \<open>\<Gamma> \<turnstile> Stmt stmt seq is ok\<close>
+    fixes stmt :: stmt
+  assumes \<open>\<Gamma> \<turnstile> (stmt # seq) is ok\<close>
     shows \<open>\<Gamma> \<turnstile> stmt is ok \<and> \<Gamma> \<turnstile> seq is ok\<close>
-  using assms by auto
+  using assms unfolding typing_is_ok_list_def typing_is_ok_stmt_def by auto
 
 lemma one_seq_typing_is_okI: 
+    fixes stmt :: stmt
   assumes \<open>\<Gamma> \<turnstile> stmt is ok\<close>
-    shows \<open>\<Gamma> \<turnstile> Stmt stmt Empty is ok\<close>
-  using assms by auto
+    shows \<open>\<Gamma> \<turnstile> [stmt] is ok\<close>
+  using assms unfolding typing_is_ok_list_def typing_is_ok_stmt_def by auto
 
 lemma one_seq_typing_is_okE: 
-  assumes \<open>\<Gamma> \<turnstile> Stmt stmt Empty is ok\<close>
+    fixes stmt :: stmt
+    assumes \<open>\<Gamma> \<turnstile> [stmt] is ok\<close>
     shows \<open>\<Gamma> \<turnstile> stmt is ok\<close>
-  using assms by auto
+  using assms unfolding typing_is_ok_list_def typing_is_ok_stmt_def by auto
 
 \<comment> \<open>Lemma aliases for the BIL specification\<close>
 
@@ -77,72 +114,72 @@ lemmas T_SEQ_REC = rec_seq_typing_is_okI
 lemma move_stmt_typing_is_okI:
   assumes \<open>\<Gamma> \<turnstile> ((id' :\<^sub>t t)::exp) :: t\<close> and \<open>\<Gamma> \<turnstile> exp :: t\<close> 
     shows \<open>\<Gamma> \<turnstile> (((id' :\<^sub>t t) := exp)::stmt) is ok\<close>
-  using assms by simp
+  using assms unfolding typing_is_ok_list_def typing_is_ok_stmt_def by simp
 
 lemma move_stmt_typing_is_okE:
   assumes \<open>\<Gamma> \<turnstile> (((id' :\<^sub>t t) := exp)::stmt) is ok\<close> 
     shows \<open>(\<Gamma> \<turnstile> ((id' :\<^sub>t t)::exp) :: t) \<and> (\<Gamma> \<turnstile> exp :: t)\<close>
-  using assms by auto
+  using assms unfolding typing_is_ok_list_def typing_is_ok_stmt_def by auto
 
 lemma jmp_stmt_typing_is_okI:
   assumes \<open>\<Gamma> \<turnstile> exp :: imm\<langle>sz\<rangle>\<close> 
     shows \<open>\<Gamma> \<turnstile> jmp exp is ok\<close>
-  using assms by auto
+  using assms unfolding typing_is_ok_list_def typing_is_ok_stmt_def by auto
 
 lemma jmp_stmt_typing_is_okE:
   assumes \<open>\<Gamma> \<turnstile> jmp exp is ok\<close> 
     shows \<open>\<exists>sz. (\<Gamma> \<turnstile> exp :: imm\<langle>sz\<rangle>)\<close>
-  using assms by auto
+  using assms unfolding typing_is_ok_list_def typing_is_ok_stmt_def by auto
 
 lemma cpuexn_stmt_typing_is_okI:
   assumes \<open>\<Gamma> is ok\<close>
     shows \<open>\<Gamma> \<turnstile> cpuexn num is ok\<close>
-  using assms by auto
+  using assms unfolding typing_is_ok_list_def typing_is_ok_stmt_def by auto
 
 lemma cpuexn_stmt_typing_is_okE:
   assumes \<open>\<Gamma> \<turnstile> cpuexn num is ok\<close>
     shows \<open>\<Gamma> is ok\<close>
-  using assms by auto
+  using assms unfolding typing_is_ok_list_def typing_is_ok_stmt_def by auto
 
 lemma special_stmt_typing_is_okI: 
   assumes \<open>\<Gamma> is ok\<close>
     shows \<open>\<Gamma> \<turnstile> special[str] is ok\<close>
-  using assms by simp
+  using assms unfolding typing_is_ok_list_def typing_is_ok_stmt_def by simp
 
 lemma special_stmt_typing_is_okE: 
   assumes \<open>\<Gamma> \<turnstile> special[str] is ok\<close>
     shows \<open>\<Gamma> is ok\<close>
-  using assms by simp
+  using assms unfolding typing_is_ok_list_def typing_is_ok_stmt_def by simp
 
 lemma while_stmt_typing_is_okI: 
   assumes \<open>\<Gamma> \<turnstile> e :: imm\<langle>1\<rangle>\<close> and \<open>\<Gamma> \<turnstile> seq is ok\<close>
     shows \<open>\<Gamma> \<turnstile> while (e) seq is ok\<close>
-  using assms by simp
+  using assms unfolding typing_is_ok_list_def typing_is_ok_stmt_def by simp
 
 lemma while_stmt_typing_is_okE: 
   assumes \<open>\<Gamma> \<turnstile> while (e) seq is ok\<close>
     shows \<open>(\<Gamma> \<turnstile> e :: imm\<langle>1\<rangle>) \<and> \<Gamma> \<turnstile> seq is ok\<close>
-  using assms by simp
+  using assms unfolding typing_is_ok_list_def typing_is_ok_stmt_def by simp
 
 lemma if_stmt_typing_is_okI: 
   assumes \<open>\<Gamma> \<turnstile> e :: imm\<langle>1\<rangle>\<close> and \<open>\<Gamma> \<turnstile> seq\<^sub>1 is ok\<close> and \<open>\<Gamma> \<turnstile> seq\<^sub>2 is ok\<close>
     shows \<open>\<Gamma> \<turnstile> if (e) seq\<^sub>1 else seq\<^sub>2 is ok\<close>
-  using assms by auto
+  using assms unfolding typing_is_ok_list_def typing_is_ok_stmt_def by auto
 
 lemma if_stmt_typing_is_okE: 
   assumes \<open>\<Gamma> \<turnstile> if (e) seq\<^sub>1 else seq\<^sub>2 is ok\<close>
     shows \<open>(\<Gamma> \<turnstile> e :: imm\<langle>1\<rangle>) \<and> \<Gamma> \<turnstile> seq\<^sub>1 is ok \<and> \<Gamma> \<turnstile> seq\<^sub>2 is ok\<close>
-  using assms by auto
+  using assms unfolding typing_is_ok_list_def typing_is_ok_stmt_def by auto
 
 lemma ifthen_stmt_typing_is_okI:
   assumes \<open>\<Gamma> \<turnstile> e :: imm\<langle>1\<rangle>\<close> and \<open>\<Gamma> \<turnstile> seq is ok\<close>
     shows \<open>\<Gamma> \<turnstile> IfThen e seq is ok\<close>
-  using assms by auto
+  using assms unfolding typing_is_ok_list_def typing_is_ok_stmt_def by auto
 
 lemma ifthen_stmt_typing_is_okE:
   assumes \<open>\<Gamma> \<turnstile> IfThen e seq is ok\<close>
     shows \<open>(\<Gamma> \<turnstile> e :: imm\<langle>1\<rangle>) \<and> \<Gamma> \<turnstile> seq is ok\<close>
-  using assms by auto
+  using assms unfolding typing_is_ok_list_def typing_is_ok_stmt_def by auto
 
 \<comment> \<open>Lemma aliases for the BIL specification\<close>
 
@@ -155,14 +192,14 @@ lemmas T_IF = if_stmt_typing_is_okI
 lemmas T_IFTHEN = ifthen_stmt_typing_is_okI
 
 method solve_T_BIL = (
-  match conclusion in
-    \<open>_ \<turnstile> bil.Empty is ok\<close> \<Rightarrow> \<open>rule T_SEQ_EMPTY, solve_TG\<close>
-  \<bar> \<open>_ \<turnstile> Stmt _ bil.Empty is ok\<close> \<Rightarrow> \<open>rule T_SEQ_ONE, solve_T_BIL\<close>
-  \<bar> \<open>_ \<turnstile> Stmt _ _ is ok\<close> \<Rightarrow> \<open>rule T_SEQ_REC, solve_T_BIL\<close>
-  \<bar> \<open>_ \<turnstile> jmp (_ \<Colon> sz) is ok\<close> for sz \<Rightarrow> \<open>rule T_JMP[of _ _ sz], solve_T_WORD\<close>
+  (rule T_SEQ_EMPTY, solve_TG) |
+  (rule T_SEQ_ONE, solve_T_BIL) |
+  (rule T_SEQ_REC, solve_T_BIL, solve_T_BIL) |
+  (match conclusion in
+    \<open>_ \<turnstile> jmp (_ \<Colon> sz) is ok\<close> for sz \<Rightarrow> \<open>rule T_JMP[of _ _ sz], solve_T_WORD\<close>
   \<bar> \<open>_ \<turnstile> (_ := _) is ok\<close> \<Rightarrow> \<open>rule T_MOVE, solve_T_VAR, solve_T_EXP\<close> 
   \<bar> \<open>_ \<turnstile> IfThen _ _ is ok\<close> \<Rightarrow> \<open>rule T_IFTHEN, solve_T_EXP, solve_T_BIL\<close>
-  \<bar> _ \<Rightarrow> \<open>succeed\<close>
+  \<bar> _ \<Rightarrow> \<open>succeed\<close>)
 )
 
 end
