extras/Simp_PC.thy
@@ -1,0 +1,75 @@
+theory Simp_PC
+  imports 
+    "../Instruction_Syntax"
+begin
+
+text \<open>
+  A program's variable state may contain duplicate variables from move statements, to prevent
+  the variable state from becoming too large we employ a simp procedure .
+      
+  We cant use fun_upd as it invokes the simplifier.      
+\<close>
+
+simproc_setup simp_pc (\<open>(\<Delta>, pc, mem)\<close>) = \<open>fn _ =>
+  let
+    fun gen_fun_upd NONE T _ _ = NONE
+      | gen_fun_upd (SOME f) T x y = SOME (Const (\<^const_name>\<open>fun_upd\<close>, T) $ f $ x $ y)
+    fun dest_fun_T1 (Type (_, T :: Ts)) = T
+    fun find_double (t as Const (\<^const_name>\<open>Product_Type.Pair\<close>,_) $ _ $ (Const (\<^const_name>\<open>Product_Type.Pair\<close>,_) $ z $ _)) =
+      let
+        val _ = Pretty.writeln (Pretty.str "pc: ")
+        val _ = Pretty.writeln (Syntax.pretty_term @{context} z)
+
+
+       (* fun find (Const (\<^const_name>\<open>Product_Type.prod\<close>,T) $ g $ v $ w) =
+              if v aconv x then SOME g else gen_fun_upd (find g) T v w
+          | find t = NONE
+      in (dest_fun_T1 T, gen_fun_upd (find f) T x y)*)
+      in (NONE) end
+
+    fun proc ctxt ct =
+      let
+        val t = Thm.term_of ct
+        val _ = Pretty.writeln (Syntax.pretty_term @{context} t)
+      in
+        (case find_double t of
+          (NONE) => NONE
+        | (SOME rhs) =>
+            SOME (Goal.prove ctxt [] [] (Logic.mk_equals (t, rhs))
+              (fn _ =>
+                 simp_tac ctxt 1
+              )
+           )
+        )
+      end
+  in proc end
+\<close>
+
+text \<open>Remove this method from the simpset to prevent it interfering\<close>
+
+declare [[simproc del: simp_pc]]
+
+ML \<open>
+
+fun simp_variable goal_target ctxt = SIMPLE_METHOD (goal_target (
+  (simp_tac (empty_simpset ctxt addsimprocs [\<^simproc>\<open>simp_pc\<close>]))));
+
+val method_setup =
+  Method.setup \<^binding>\<open>simp_pc\<close>
+    (Scan.succeed (simp_variable HEADGOAL))
+    "simplification" #>
+  Method.setup \<^binding>\<open>simp_all_pc\<close>
+    (Scan.succeed (simp_variable ALLGOALS))
+    "simplification (all goals)";
+
+val _ =
+  Theory.setup method_setup;
+\<close>
+
+
+lemma "(\<Delta>, (12::nat) mod 9, mem) = (\<Delta>, z, mem)"
+  apply simp_pc
+  using [[simp_trace_new]] apply simp
+
+
+end
